<?xml version="1.0"?>
<rdf:RDF xmlns="http://w3.id.org/def/BibliOWL#"
     xml:base="http://w3.id.org/def/BibliOWL"
     xmlns:dc="http://purl.org/dc/elements/1.1/"
     xmlns:cis="http://dati.beniculturali.it/cis/"
     xmlns:def="http://datos.bne.es/def/"
     xmlns:obo="http://purl.obolibrary.org/obo/"
     xmlns:owl="http://www.w3.org/2002/07/owl#"
     xmlns:rdf="http://www.w3.org/1999/02/22-rdf-syntax-ns#"
     xmlns:xml="http://www.w3.org/XML/1998/namespace"
     xmlns:xsd="http://www.w3.org/2001/XMLSchema#"
     xmlns:rdfs="http://www.w3.org/2000/01/rdf-schema#"
     xmlns:BibliOWL="http://w3.id.org/def/BibliOWL#">
    <owl:Ontology rdf:about="http://w3.id.org/def/BibliOWL#">
        <owl:imports rdf:resource="http://datos.bne.es/def/"/>
        <dc:creator>Lucía Martín Fernández</dc:creator>
        <dc:creator>Álvaro González Berdasco</dc:creator>
        <dc:date>2023-01-25</dc:date>
        <dc:description xml:lang="en">The BibliOWL ontology has been created to connect information about the physical Libraries and the content of its catalogues. 

The general goal of the BibliOWL ontology is to model data about libraries regarding its location, organization, provided services and administration, together with its users and the description of its catalogue. The catalogue is composed by different items corresponding to various resources related to different creative works expressions. The ontology includes information about the characteristics of this contents. The class loan relates users with items so that the library&apos;s content movement can be tracked.</dc:description>
        <dc:license rdf:resource="http://creativecommons.org/licenses/by/3.0/it/"/>
        <dc:rights rdf:resource="http://creativecommons.org/licenses/by/3.0/it/legalcode"/>
        <dc:title>BibliOWL</dc:title>
        <rdfs:comment xml:lang="en">The BibliOWL ontology has been created as part of the Final Assigment for the Semanthic Technologies course of the Master&apos;s in Computational Biology of Universidad Politécnica de Madrid, in the academical year 2022-2023.</rdfs:comment>
        <owl:versionInfo xml:lang="en">Version 1.0 - 25 January 2023</owl:versionInfo>
    </owl:Ontology>
    


    <!-- 
    ///////////////////////////////////////////////////////////////////////////////////////
    //
    // Annotation properties
    //
    ///////////////////////////////////////////////////////////////////////////////////////
     -->


    


    <!-- http://purl.org/dc/elements/1.1/creator -->


    <owl:AnnotationProperty rdf:about="http://purl.org/dc/elements/1.1/creator"/>
    


    <!-- http://purl.org/dc/elements/1.1/date -->


    <owl:AnnotationProperty rdf:about="http://purl.org/dc/elements/1.1/date"/>
    


    <!-- http://purl.org/dc/elements/1.1/description -->


    <owl:AnnotationProperty rdf:about="http://purl.org/dc/elements/1.1/description"/>
    


    <!-- http://purl.org/dc/elements/1.1/license -->


    <owl:AnnotationProperty rdf:about="http://purl.org/dc/elements/1.1/license"/>
    


    <!-- http://purl.org/dc/elements/1.1/modified -->


    <owl:AnnotationProperty rdf:about="http://purl.org/dc/elements/1.1/modified"/>
    


    <!-- http://purl.org/dc/elements/1.1/rights -->


    <owl:AnnotationProperty rdf:about="http://purl.org/dc/elements/1.1/rights"/>
    


    <!-- http://purl.org/dc/elements/1.1/title -->


    <owl:AnnotationProperty rdf:about="http://purl.org/dc/elements/1.1/title"/>
    


    <!-- http://www.w3.org/2000/01/rdf-schema#comment -->


    <owl:AnnotationProperty rdf:about="http://www.w3.org/2000/01/rdf-schema#comment"/>
    


    <!-- http://www.w3.org/2000/01/rdf-schema#isDefinedBy -->


    <owl:AnnotationProperty rdf:about="http://www.w3.org/2000/01/rdf-schema#isDefinedBy"/>
    


    <!-- http://www.w3.org/2000/01/rdf-schema#label -->


    <owl:AnnotationProperty rdf:about="http://www.w3.org/2000/01/rdf-schema#label"/>
    


    <!-- http://www.w3.org/2002/07/owl#versionInfo -->


    <owl:AnnotationProperty rdf:about="http://www.w3.org/2002/07/owl#versionInfo"/>
    


    <!-- 
    ///////////////////////////////////////////////////////////////////////////////////////
    //
    // Datatypes
    //
    ///////////////////////////////////////////////////////////////////////////////////////
     -->


    


    <!-- http://www.w3.org/1999/02/22-rdf-syntax-ns#PlainLiteral -->


    <rdfs:Datatype rdf:about="http://www.w3.org/1999/02/22-rdf-syntax-ns#PlainLiteral"/>
    


    <!-- http://www.w3.org/2000/01/rdf-schema#Literal -->


    <rdfs:Datatype rdf:about="http://www.w3.org/2000/01/rdf-schema#Literal"/>
    


    <!-- http://www.w3.org/2001/XMLSchema#date -->


    <rdfs:Datatype rdf:about="http://www.w3.org/2001/XMLSchema#date"/>
    


    <!-- http://www.w3.org/2001/XMLSchema#decimal -->


    <rdfs:Datatype rdf:about="http://www.w3.org/2001/XMLSchema#decimal"/>
    


    <!-- http://www.w3.org/2001/XMLSchema#float -->


    <rdfs:Datatype rdf:about="http://www.w3.org/2001/XMLSchema#float"/>
    


    <!-- http://www.w3.org/2001/XMLSchema#time -->


    <rdfs:Datatype rdf:about="http://www.w3.org/2001/XMLSchema#time"/>
    


    <!-- 
    ///////////////////////////////////////////////////////////////////////////////////////
    //
    // Object Properties
    //
    ///////////////////////////////////////////////////////////////////////////////////////
     -->


    


    <!-- http://dati.beniculturali.it/cis/accessConditionFor -->


    <owl:ObjectProperty rdf:about="http://dati.beniculturali.it/cis/accessConditionFor">
        <owl:inverseOf rdf:resource="http://dati.beniculturali.it/cis/hasAccessCondition"/>
        <rdfs:domain rdf:resource="http://dati.beniculturali.it/cis/AccessCondition"/>
        <rdfs:range rdf:resource="http://dati.beniculturali.it/cis/CulturalInstituteOrSite"/>
        <rdfs:comment xml:lang="en">Inverse property of &quot;has access condition&quot;</rdfs:comment>
        <rdfs:comment xml:lang="it">Proprietà inversa di &quot;ha condizione di accesso&quot;</rdfs:comment>
        <rdfs:isDefinedBy rdf:resource="http://dati.beniculturali.it/cis/"/>
        <rdfs:label xml:lang="en">access condition for</rdfs:label>
        <rdfs:label xml:lang="it">condizione di accesso per</rdfs:label>
    </owl:ObjectProperty>
    


    <!-- http://dati.beniculturali.it/cis/available -->


    <owl:ObjectProperty rdf:about="http://dati.beniculturali.it/cis/available">
        <rdfs:domain rdf:resource="http://dati.beniculturali.it/cis/ContactPoint"/>
        <rdfs:range rdf:resource="http://dati.beniculturali.it/cis/OpeningHoursSpecification"/>
        <rdfs:comment xml:lang="en">Property used to associate a contact point with hours specification in which the contact point is available.</rdfs:comment>
        <rdfs:comment xml:lang="it">Proprietà utilizzata per associare  un punto di contatto a fasce orarie in cui il punto di contatto è disponibile.</rdfs:comment>
        <rdfs:isDefinedBy rdf:resource="http://dati.beniculturali.it/cis/"/>
        <rdfs:label xml:lang="en">available</rdfs:label>
        <rdfs:label xml:lang="it">disponibile</rdfs:label>
        <owl:versionInfo xml:lang="it">stabile</owl:versionInfo>
        <owl:versionInfo xml:lang="en">stable</owl:versionInfo>
    </owl:ObjectProperty>
    


    <!-- http://dati.beniculturali.it/cis/catalogue -->


    <owl:ObjectProperty rdf:about="http://dati.beniculturali.it/cis/catalogue">
        <owl:inverseOf rdf:resource="http://dati.beniculturali.it/cis/isCatalogueOf"/>
        <rdfs:domain rdf:resource="http://dati.beniculturali.it/cis/CulturalInstituteOrSite"/>
        <rdfs:range rdf:resource="http://dati.beniculturali.it/cis/Catalogue"/>
        <rdfs:comment xml:lang="en">Property used to associate the Cultural Institute or SIte with a catalogue of cultural collections included in the institute or site. The relatioships can be used to indicate that a Cultural Institute or Site has an its own catalogue or situations where a Cultural Institute or Site contributes to a union catalogue (this latter case is represented by libraries that can contribute to or participate in a union catalogue).</rdfs:comment>
        <rdfs:comment xml:lang="it">Proprietà utilizzata per associare l&apos;istituto e luogo della cultura a un  catalogo che descrive le opere in esso contenute. Tale relazione può essere utilizzata per indicare che un istituto e luogo della cultura ha un catalogo ma anche una situazione per cui un istituto e luogo della cultura partecipa a un catalogo (in quest&apos;ultimo caso un esempio è rappresentato dalle biblioteche che possono partecipare a un catalogo collettivo).</rdfs:comment>
        <rdfs:isDefinedBy rdf:resource="http://dati.beniculturali.it/cis/"/>
        <rdfs:label xml:lang="it">catalogo</rdfs:label>
        <rdfs:label xml:lang="en">catalogue</rdfs:label>
        <owl:versionInfo xml:lang="it">stabile</owl:versionInfo>
        <owl:versionInfo>stable</owl:versionInfo>
    </owl:ObjectProperty>
    


    <!-- http://dati.beniculturali.it/cis/hasAccessCondition -->


    <owl:ObjectProperty rdf:about="http://dati.beniculturali.it/cis/hasAccessCondition">
        <rdfs:domain rdf:resource="http://dati.beniculturali.it/cis/CulturalInstituteOrSite"/>
        <rdfs:range rdf:resource="http://dati.beniculturali.it/cis/AccessCondition"/>
        <rdfs:comment xml:lang="en">Property used to associate the Cultural Institute or Site or the Event with its access condition information</rdfs:comment>
        <rdfs:comment xml:lang="it">Proprietà utilizzata per associare l&apos;istituto e luogo della cultura o l&apos;evento con le condizioni di accesso.</rdfs:comment>
        <rdfs:isDefinedBy rdf:resource="http://dati.beniculturali.it/cis/"/>
        <rdfs:label xml:lang="it">ha condizioni di accesso</rdfs:label>
        <rdfs:label xml:lang="en">has access condition</rdfs:label>
        <owl:versionInfo xml:lang="it">stabile</owl:versionInfo>
        <owl:versionInfo>stable</owl:versionInfo>
    </owl:ObjectProperty>
    


    <!-- http://dati.beniculturali.it/cis/hasAddress -->


    <owl:ObjectProperty rdf:about="http://dati.beniculturali.it/cis/hasAddress">
        <rdfs:domain rdf:resource="http://dati.beniculturali.it/cis/Site"/>
        <rdfs:range rdf:resource="http://dati.beniculturali.it/cis/Address"/>
        <rdfs:comment xml:lang="en">Property that permits to associate a site with an address</rdfs:comment>
        <rdfs:comment xml:lang="it">Proprietà che consente di associare un sito fisico a un indirizzo.</rdfs:comment>
        <rdfs:isDefinedBy rdf:resource="http://dati.beniculturali.it/cis/"/>
        <rdfs:label xml:lang="it">ha indirizzo</rdfs:label>
        <rdfs:label xml:lang="en">has address</rdfs:label>
        <owl:versionInfo xml:lang="it">stabile</owl:versionInfo>
        <owl:versionInfo>stable</owl:versionInfo>
    </owl:ObjectProperty>
    


    <!-- http://dati.beniculturali.it/cis/hasContactPoint -->


    <owl:ObjectProperty rdf:about="http://dati.beniculturali.it/cis/hasContactPoint">
        <rdfs:domain rdf:resource="http://dati.beniculturali.it/cis/CulturalInstituteOrSite"/>
        <rdfs:range rdf:resource="http://dati.beniculturali.it/cis/ContactPoint"/>
        <rdfs:comment xml:lang="en">Property which links a cultural insttiute or site to its contact points. The same property is used to link in a similar way the event to its contact points and to link the site of the cultural institute or site with its contact points</rdfs:comment>
        <rdfs:comment xml:lang="it">Proprietà che collega un istituto e luogo della cultura ai propri punti di contatto. La stessa proprietà è utilizzata in maniera analoga per collegare il luogo fisico con i propri punti di contatto, ad anche per collegare un evento ai propri contatti</rdfs:comment>
        <rdfs:isDefinedBy rdf:resource="http://dati.beniculturali.it/cis/"/>
        <rdfs:label xml:lang="it">ha punto di contatto</rdfs:label>
        <rdfs:label xml:lang="en">has contact point</rdfs:label>
        <owl:versionInfo xml:lang="it">stabile</owl:versionInfo>
        <owl:versionInfo>stable</owl:versionInfo>
    </owl:ObjectProperty>
    


    <!-- http://dati.beniculturali.it/cis/hasDayOfWeek -->


    <owl:ObjectProperty rdf:about="http://dati.beniculturali.it/cis/hasDayOfWeek">
        <owl:inverseOf rdf:resource="http://dati.beniculturali.it/cis/isDayOfWeekOf"/>
        <rdfs:domain rdf:resource="http://dati.beniculturali.it/cis/OpeningHoursSpecification"/>
        <rdfs:range rdf:resource="http://dati.beniculturali.it/cis/DayOfWeek"/>
        <rdfs:comment xml:lang="it">Questa proprietà è utilizzata per specificare gli orari di apertura e in particolare i giorni della settimana.</rdfs:comment>
        <rdfs:comment xml:lang="en">This property is used to specify the opening hours and in particular the days of the week.</rdfs:comment>
        <rdfs:isDefinedBy rdf:resource="http://dati.beniculturali.it/cis/"/>
        <rdfs:label xml:lang="it">ha giorno della settimana </rdfs:label>
        <rdfs:label xml:lang="en">has day of week </rdfs:label>
        <owl:versionInfo xml:lang="en">unstable</owl:versionInfo>
        <owl:versionInfo xml:lang="it">versione non definitiva</owl:versionInfo>
    </owl:ObjectProperty>
    


    <!-- http://dati.beniculturali.it/cis/hasGeographicalLocation -->


    <owl:ObjectProperty rdf:about="http://dati.beniculturali.it/cis/hasGeographicalLocation">
        <rdfs:domain rdf:resource="http://dati.beniculturali.it/cis/Site"/>
        <rdfs:range rdf:resource="http://dati.beniculturali.it/cis/GeographicalFeature"/>
        <rdfs:comment xml:lang="en">Property used to associate a site with a geographical area where the site is located.</rdfs:comment>
        <rdfs:comment xml:lang="it">Proprietà che consente di associare una sede di un istituto e luogo della cultura a un&apos;area geografica in cui si trova la sede.</rdfs:comment>
        <rdfs:isDefinedBy rdf:resource="http://dati.beniculturali.it/cis/"/>
        <rdfs:label xml:lang="it">ha locazione geografica</rdfs:label>
        <rdfs:label xml:lang="en">has geographical location</rdfs:label>
        <owl:versionInfo xml:lang="it">stabile</owl:versionInfo>
        <owl:versionInfo>stable</owl:versionInfo>
    </owl:ObjectProperty>
    


    <!-- http://dati.beniculturali.it/cis/hasGeometry -->


    <owl:ObjectProperty rdf:about="http://dati.beniculturali.it/cis/hasGeometry">
        <rdfs:domain rdf:resource="http://dati.beniculturali.it/cis/Site"/>
        <rdfs:range rdf:resource="http://dati.beniculturali.it/cis/Geometry"/>
        <rdfs:comment xml:lang="en">Property used to associate a site with its own geographical coordinates</rdfs:comment>
        <rdfs:comment xml:lang="it">Proprietà utilizzata per associare un sito alle proprie coordinate geografiche.</rdfs:comment>
        <rdfs:isDefinedBy rdf:resource="http://dati.beniculturali.it/cis/"/>
        <rdfs:label xml:lang="it">ha geometria</rdfs:label>
        <rdfs:label xml:lang="en">has geometry</rdfs:label>
        <owl:versionInfo xml:lang="it">stabile</owl:versionInfo>
        <owl:versionInfo>stable</owl:versionInfo>
    </owl:ObjectProperty>
    


    <!-- http://dati.beniculturali.it/cis/hasSite -->


    <owl:ObjectProperty rdf:about="http://dati.beniculturali.it/cis/hasSite">
        <owl:inverseOf rdf:resource="http://dati.beniculturali.it/cis/isSiteOf"/>
        <rdfs:domain rdf:resource="http://dati.beniculturali.it/cis/CulturalInstituteOrSite"/>
        <rdfs:range rdf:resource="http://dati.beniculturali.it/cis/Site"/>
        <rdfs:comment xml:lang="en">Property which links a cultural institute or site to its own physical site(s).</rdfs:comment>
        <rdfs:comment xml:lang="it">Proprietà che collega un istituto e luogo della cultura al proprio o ai propri siti fisici.</rdfs:comment>
        <rdfs:isDefinedBy rdf:resource="http://dati.beniculturali.it/cis/"/>
        <rdfs:label xml:lang="it">ha contenitore fisico</rdfs:label>
        <rdfs:label xml:lang="it">ha sede</rdfs:label>
        <rdfs:label xml:lang="en">has site</rdfs:label>
        <owl:versionInfo xml:lang="it">stabile</owl:versionInfo>
        <owl:versionInfo>stable</owl:versionInfo>
    </owl:ObjectProperty>
    


    <!-- http://dati.beniculturali.it/cis/isCatalogueOf -->


    <owl:ObjectProperty rdf:about="http://dati.beniculturali.it/cis/isCatalogueOf">
        <rdfs:domain rdf:resource="http://dati.beniculturali.it/cis/Catalogue"/>
        <rdfs:range rdf:resource="http://dati.beniculturali.it/cis/CulturalInstituteOrSite"/>
        <rdfs:comment xml:lang="en">Inverse property of &quot;has catalogue&quot;.</rdfs:comment>
        <rdfs:comment xml:lang="it">Proprietà inversa di &quot;ha catalogo&quot;.</rdfs:comment>
        <rdfs:isDefinedBy rdf:resource="http://dati.beniculturali.it/cis/"/>
        <rdfs:label xml:lang="en">is catalogue of</rdfs:label>
        <rdfs:label xml:lang="it">è catalogo di</rdfs:label>
        <owl:versionInfo xml:lang="en">unstable</owl:versionInfo>
        <owl:versionInfo xml:lang="it">versione non definitiva</owl:versionInfo>
    </owl:ObjectProperty>
    


    <!-- http://dati.beniculturali.it/cis/isDayOfWeekOf -->


    <owl:ObjectProperty rdf:about="http://dati.beniculturali.it/cis/isDayOfWeekOf">
        <rdfs:domain rdf:resource="http://dati.beniculturali.it/cis/DayOfWeek"/>
        <rdfs:range rdf:resource="http://dati.beniculturali.it/cis/OpeningHoursSpecification"/>
        <rdfs:comment xml:lang="en">Inverse property of has day of week.</rdfs:comment>
        <rdfs:comment xml:lang="it">Proprietà inversa di &quot;ha giorno della settimana&quot;.</rdfs:comment>
        <rdfs:isDefinedBy rdf:resource="http://dati.beniculturali.it/cis/"/>
        <rdfs:label xml:lang="en">is day of week of </rdfs:label>
        <rdfs:label xml:lang="it">è giorno della settimana di </rdfs:label>
        <owl:versionInfo xml:lang="en">unstable</owl:versionInfo>
        <owl:versionInfo xml:lang="it">versione non definitiva</owl:versionInfo>
    </owl:ObjectProperty>
    


    <!-- http://dati.beniculturali.it/cis/isProvidedBy -->


    <owl:ObjectProperty rdf:about="http://dati.beniculturali.it/cis/isProvidedBy">
        <owl:inverseOf rdf:resource="http://dati.beniculturali.it/cis/providesService"/>
        <rdfs:domain rdf:resource="http://dati.beniculturali.it/cis/Service"/>
        <rdfs:range rdf:resource="http://dati.beniculturali.it/cis/CulturalInstituteOrSite"/>
        <rdfs:comment xml:lang="en">Inverse property of &quot;provides service&quot;</rdfs:comment>
        <rdfs:comment xml:lang="it">Proprietà inversa di &quot;fornisce servizio&quot;</rdfs:comment>
        <rdfs:isDefinedBy rdf:resource="http://dati.beniculturali.it/cis/"/>
        <rdfs:label xml:lang="en">is provided by</rdfs:label>
        <rdfs:label xml:lang="it">è fornito da</rdfs:label>
    </owl:ObjectProperty>
    


    <!-- http://dati.beniculturali.it/cis/isSiteOf -->


    <owl:ObjectProperty rdf:about="http://dati.beniculturali.it/cis/isSiteOf">
        <rdfs:domain rdf:resource="http://dati.beniculturali.it/cis/Site"/>
        <rdfs:range rdf:resource="http://dati.beniculturali.it/cis/CulturalInstituteOrSite"/>
        <rdfs:comment xml:lang="en">Inverse property of &quot;has Site&quot;</rdfs:comment>
        <rdfs:comment xml:lang="it">Proprietà inversa di &quot;ha sede&quot;.</rdfs:comment>
        <rdfs:isDefinedBy rdf:resource="http://dati.beniculturali.it/cis/"/>
        <rdfs:label xml:lang="en">is site of</rdfs:label>
        <rdfs:label xml:lang="it">è contenitore fisico di</rdfs:label>
        <rdfs:label xml:lang="it">è sede di</rdfs:label>
        <owl:versionInfo xml:lang="it">stabile</owl:versionInfo>
        <owl:versionInfo xml:lang="en">stable</owl:versionInfo>
    </owl:ObjectProperty>
    


    <!-- http://dati.beniculturali.it/cis/providesService -->


    <owl:ObjectProperty rdf:about="http://dati.beniculturali.it/cis/providesService">
        <rdfs:domain rdf:resource="http://dati.beniculturali.it/cis/CulturalInstituteOrSite"/>
        <rdfs:range rdf:resource="http://dati.beniculturali.it/cis/Service"/>
        <rdfs:comment xml:lang="en">Property used to represent a supply service relationship between a cultural institute or site and a service.</rdfs:comment>
        <rdfs:comment xml:lang="it">Proprietà utilizzata per rappresentare una relazione di fornitura di servizi da parte di un istituto e luogo della cultura.</rdfs:comment>
        <rdfs:isDefinedBy rdf:resource="http://dati.beniculturali.it/cis/"/>
        <rdfs:label xml:lang="it">fornisce servizi</rdfs:label>
        <rdfs:label xml:lang="en">provides Service</rdfs:label>
        <owl:versionInfo xml:lang="it">stabile</owl:versionInfo>
        <owl:versionInfo>stable</owl:versionInfo>
    </owl:ObjectProperty>
    


    <!-- http://datos.bne.es/def/OP1001 -->


    <owl:ObjectProperty rdf:about="http://datos.bne.es/def/OP1001">
        <owl:inverseOf rdf:resource="http://datos.bne.es/def/OP5001"/>
        <rdfs:domain rdf:resource="http://datos.bne.es/def/C1001"/>
        <rdfs:range rdf:resource="http://datos.bne.es/def/C1005"/>
        <rdfs:label xml:lang="en">is created by (person)</rdfs:label>
    </owl:ObjectProperty>
    


    <!-- http://datos.bne.es/def/OP1002 -->


    <owl:ObjectProperty rdf:about="http://datos.bne.es/def/OP1002">
        <owl:inverseOf rdf:resource="http://datos.bne.es/def/OP2002"/>
        <rdfs:domain rdf:resource="http://datos.bne.es/def/C1001"/>
        <rdfs:range rdf:resource="http://datos.bne.es/def/C1002"/>
        <rdfs:label xml:lang="en">is realized through</rdfs:label>
    </owl:ObjectProperty>
    


    <!-- http://datos.bne.es/def/OP1005 -->


    <owl:ObjectProperty rdf:about="http://datos.bne.es/def/OP1005">
        <owl:inverseOf rdf:resource="http://datos.bne.es/def/OP6001"/>
        <rdfs:domain rdf:resource="http://datos.bne.es/def/C1001"/>
        <rdfs:range rdf:resource="http://datos.bne.es/def/C1006"/>
        <rdfs:label xml:lang="en">is created by (corporate body)</rdfs:label>
    </owl:ObjectProperty>
    


    <!-- http://datos.bne.es/def/OP2001 -->


    <owl:ObjectProperty rdf:about="http://datos.bne.es/def/OP2001">
        <owl:inverseOf rdf:resource="http://datos.bne.es/def/OP3002"/>
        <rdfs:domain rdf:resource="http://datos.bne.es/def/C1002"/>
        <rdfs:range rdf:resource="http://datos.bne.es/def/C1003"/>
        <rdfs:label xml:lang="en">is embodied in</rdfs:label>
    </owl:ObjectProperty>
    


    <!-- http://datos.bne.es/def/OP2002 -->


    <owl:ObjectProperty rdf:about="http://datos.bne.es/def/OP2002">
        <rdfs:domain rdf:resource="http://datos.bne.es/def/C1002"/>
        <rdfs:range rdf:resource="http://datos.bne.es/def/C1001"/>
        <rdfs:label xml:lang="en">is realization of</rdfs:label>
    </owl:ObjectProperty>
    


    <!-- http://datos.bne.es/def/OP3001 -->


    <owl:ObjectProperty rdf:about="http://datos.bne.es/def/OP3001">
        <owl:inverseOf rdf:resource="http://datos.bne.es/def/OP4001"/>
        <rdfs:domain rdf:resource="http://datos.bne.es/def/C1003"/>
        <rdfs:range rdf:resource="http://datos.bne.es/def/C1004"/>
        <rdfs:label xml:lang="en">is exemplified by</rdfs:label>
    </owl:ObjectProperty>
    


    <!-- http://datos.bne.es/def/OP3002 -->


    <owl:ObjectProperty rdf:about="http://datos.bne.es/def/OP3002">
        <rdfs:domain rdf:resource="http://datos.bne.es/def/C1003"/>
        <rdfs:range rdf:resource="http://datos.bne.es/def/C1002"/>
        <rdfs:label xml:lang="en">is embodiment of</rdfs:label>
    </owl:ObjectProperty>
    


    <!-- http://datos.bne.es/def/OP3003 -->


    <owl:ObjectProperty rdf:about="http://datos.bne.es/def/OP3003">
        <owl:inverseOf rdf:resource="http://datos.bne.es/def/OP5002"/>
        <rdfs:domain rdf:resource="http://datos.bne.es/def/C1003"/>
        <rdfs:range rdf:resource="http://datos.bne.es/def/C1005"/>
        <rdfs:label xml:lang="es">es creado (recurso) por (persona)</rdfs:label>
        <rdfs:label xml:lang="en">is created (resource) by (person)</rdfs:label>
    </owl:ObjectProperty>
    


    <!-- http://datos.bne.es/def/OP3004 -->


    <owl:ObjectProperty rdf:about="http://datos.bne.es/def/OP3004">
        <owl:inverseOf rdf:resource="http://datos.bne.es/def/OP6004"/>
        <rdfs:domain rdf:resource="http://datos.bne.es/def/C1003"/>
        <rdfs:range rdf:resource="http://datos.bne.es/def/C1006"/>
        <rdfs:label xml:lang="en">is created (resource) by (corporate body)</rdfs:label>
    </owl:ObjectProperty>
    


    <!-- http://datos.bne.es/def/OP3005 -->


    <owl:ObjectProperty rdf:about="http://datos.bne.es/def/OP3005">
        <owl:inverseOf rdf:resource="http://datos.bne.es/def/OP3006"/>
        <rdfs:domain rdf:resource="http://datos.bne.es/def/C1005"/>
        <rdfs:range rdf:resource="http://datos.bne.es/def/C1003"/>
        <rdfs:comment xml:lang="es">Relaciona una persona con un recurso con la que tiene un grado de responsabilidad no determinado (traductor, ilustrador, editor literario, coautor)</rdfs:comment>
        <rdfs:comment xml:lang="en">Relates a person with a resource that involves an uncertain degree of responsability (translator, illustrator, editor, co-author)</rdfs:comment>
        <rdfs:label xml:lang="en">contributes (person) to (resource)</rdfs:label>
    </owl:ObjectProperty>
    


    <!-- http://datos.bne.es/def/OP3006 -->


    <owl:ObjectProperty rdf:about="http://datos.bne.es/def/OP3006">
        <rdfs:domain rdf:resource="http://datos.bne.es/def/C1003"/>
        <rdfs:range rdf:resource="http://datos.bne.es/def/C1005"/>
        <rdfs:label xml:lang="en">has contributor</rdfs:label>
    </owl:ObjectProperty>
    


    <!-- http://datos.bne.es/def/OP4001 -->


    <owl:ObjectProperty rdf:about="http://datos.bne.es/def/OP4001">
        <rdfs:domain rdf:resource="http://datos.bne.es/def/C1004"/>
        <rdfs:range rdf:resource="http://datos.bne.es/def/C1003"/>
        <rdfs:label xml:lang="en">is exemplar of</rdfs:label>
    </owl:ObjectProperty>
    


    <!-- http://datos.bne.es/def/OP5001 -->


    <owl:ObjectProperty rdf:about="http://datos.bne.es/def/OP5001">
        <rdfs:domain rdf:resource="http://datos.bne.es/def/C1005"/>
        <rdfs:range rdf:resource="http://datos.bne.es/def/C1001"/>
        <rdfs:label xml:lang="en">is creator of (person)</rdfs:label>
    </owl:ObjectProperty>
    


    <!-- http://datos.bne.es/def/OP5002 -->


    <owl:ObjectProperty rdf:about="http://datos.bne.es/def/OP5002">
        <rdfs:domain rdf:resource="http://datos.bne.es/def/C1005"/>
        <rdfs:range rdf:resource="http://datos.bne.es/def/C1003"/>
        <rdfs:label xml:lang="en">is creator (person) of (resource)</rdfs:label>
    </owl:ObjectProperty>
    


    <!-- http://datos.bne.es/def/OP6001 -->


    <owl:ObjectProperty rdf:about="http://datos.bne.es/def/OP6001">
        <rdfs:domain rdf:resource="http://datos.bne.es/def/C1006"/>
        <rdfs:range rdf:resource="http://datos.bne.es/def/C1001"/>
        <rdfs:label xml:lang="en">is creator (corporate body) of</rdfs:label>
    </owl:ObjectProperty>
    


    <!-- http://datos.bne.es/def/OP6004 -->


    <owl:ObjectProperty rdf:about="http://datos.bne.es/def/OP6004">
        <rdfs:domain rdf:resource="http://datos.bne.es/def/C1006"/>
        <rdfs:range rdf:resource="http://datos.bne.es/def/C1003"/>
        <rdfs:label xml:lang="en">is creator (corporate body) of (resource)</rdfs:label>
    </owl:ObjectProperty>
    


    <!-- http://purl.obolibrary.org/obo/BFO_0000050 -->


    <owl:ObjectProperty rdf:about="http://purl.obolibrary.org/obo/BFO_0000050">
        <owl:inverseOf rdf:resource="http://purl.obolibrary.org/obo/BFO_0000051"/>
        <rdf:type rdf:resource="http://www.w3.org/2002/07/owl#TransitiveProperty"/>
        <rdfs:domain rdf:resource="http://www.w3.org/2002/07/owl#Thing"/>
        <rdfs:range rdf:resource="http://www.w3.org/2002/07/owl#Thing"/>
        <rdfs:comment xml:lang="en">a core relation that holds between a part and its whole</rdfs:comment>
        <rdfs:isDefinedBy>http://purl.obolibrary.org/obo/</rdfs:isDefinedBy>
        <rdfs:label xml:lang="en">part of</rdfs:label>
    </owl:ObjectProperty>
    


    <!-- http://purl.obolibrary.org/obo/BFO_0000051 -->


    <owl:ObjectProperty rdf:about="http://purl.obolibrary.org/obo/BFO_0000051">
        <rdf:type rdf:resource="http://www.w3.org/2002/07/owl#TransitiveProperty"/>
        <rdfs:domain rdf:resource="http://www.w3.org/2002/07/owl#Thing"/>
        <rdfs:range rdf:resource="http://www.w3.org/2002/07/owl#Thing"/>
        <rdfs:comment xml:lang="en">inverse property of &quot;part of&quot;</rdfs:comment>
        <rdfs:isDefinedBy>http://purl.obolibrary.org/obo/</rdfs:isDefinedBy>
        <rdfs:label xml:lang="en">has part</rdfs:label>
    </owl:ObjectProperty>
    


    <!-- http://w3.id.org/def/BibliOWL#contains -->


    <owl:ObjectProperty rdf:about="http://w3.id.org/def/BibliOWL#contains">
        <owl:inverseOf rdf:resource="http://w3.id.org/def/BibliOWL#isContainedIn"/>
        <rdfs:domain rdf:resource="http://dati.beniculturali.it/cis/Catalogue"/>
        <rdfs:range rdf:resource="http://datos.bne.es/def/C1004"/>
        <rdfs:isDefinedBy>http://w3.id.org/def/BibliOWL#</rdfs:isDefinedBy>
        <rdfs:label xml:lang="en">(catalogue) contains (item)</rdfs:label>
    </owl:ObjectProperty>
    


    <!-- http://w3.id.org/def/BibliOWL#hasMember -->


    <owl:ObjectProperty rdf:about="http://w3.id.org/def/BibliOWL#hasMember">
        <rdfs:subPropertyOf rdf:resource="http://www.w3.org/2002/07/owl#topObjectProperty"/>
        <owl:inverseOf rdf:resource="http://w3.id.org/def/BibliOWL#isMemberOf"/>
        <rdfs:domain rdf:resource="http://datos.bne.es/def/C1006"/>
        <rdfs:range rdf:resource="http://datos.bne.es/def/C1005"/>
        <rdfs:label xml:lang="en">has member</rdfs:label>
        <rdfs:label xml:lang="es">tiene miembro</rdfs:label>
    </owl:ObjectProperty>
    


    <!-- http://w3.id.org/def/BibliOWL#hasTimeInterval -->


    <owl:ObjectProperty rdf:about="http://w3.id.org/def/BibliOWL#hasTimeInterval">
        <rdfs:domain rdf:resource="http://dati.beniculturali.it/cis/TemporaryClosure"/>
        <rdfs:range rdf:resource="http://dati.beniculturali.it/cis/TimeInterval"/>
        <rdfs:isDefinedBy>http://w3.id.org/def/BibliOWL#</rdfs:isDefinedBy>
        <rdfs:label>has time interval</rdfs:label>
    </owl:ObjectProperty>
    


    <!-- http://w3.id.org/def/BibliOWL#hasUser -->


    <owl:ObjectProperty rdf:about="http://w3.id.org/def/BibliOWL#hasUser">
        <owl:inverseOf rdf:resource="http://w3.id.org/def/BibliOWL#isUserOf"/>
        <rdfs:domain rdf:resource="http://dati.beniculturali.it/cis/CulturalInstituteOrSite"/>
        <rdfs:range rdf:resource="http://w3.id.org/def/BibliOWL#User"/>
        <rdfs:isDefinedBy>http://w3.id.org/def/BibliOWL#</rdfs:isDefinedBy>
        <rdfs:label xml:lang="en">has User</rdfs:label>
    </owl:ObjectProperty>
    


    <!-- http://w3.id.org/def/BibliOWL#hasUserType -->


    <owl:ObjectProperty rdf:about="http://w3.id.org/def/BibliOWL#hasUserType">
        <rdfs:domain rdf:resource="http://w3.id.org/def/BibliOWL#User"/>
        <rdfs:range rdf:resource="http://w3.id.org/def/BibliOWL#UserType"/>
        <rdfs:isDefinedBy>http://w3.id.org/def/BibliOWL#</rdfs:isDefinedBy>
        <rdfs:label xml:lang="en">has user type</rdfs:label>
    </owl:ObjectProperty>
    


    <!-- http://w3.id.org/def/BibliOWL#isBorrowedAtLoan -->


    <owl:ObjectProperty rdf:about="http://w3.id.org/def/BibliOWL#isBorrowedAtLoan">
        <rdfs:domain rdf:resource="http://datos.bne.es/def/C1004"/>
        <rdfs:range rdf:resource="http://w3.id.org/def/BibliOWL#Loan"/>
        <rdfs:isDefinedBy>http://w3.id.org/def/BibliOWL#</rdfs:isDefinedBy>
        <rdfs:label xml:lang="en">(item) is borrowed at loan</rdfs:label>
    </owl:ObjectProperty>
    


    <!-- http://w3.id.org/def/BibliOWL#isContainedIn -->


    <owl:ObjectProperty rdf:about="http://w3.id.org/def/BibliOWL#isContainedIn">
        <rdfs:domain rdf:resource="http://datos.bne.es/def/C1004"/>
        <rdfs:range rdf:resource="http://dati.beniculturali.it/cis/Catalogue"/>
        <rdfs:isDefinedBy>http://w3.id.org/def/BibliOWL#</rdfs:isDefinedBy>
        <rdfs:label xml:lang="en">(item) is contained in (catalogue)</rdfs:label>
    </owl:ObjectProperty>
    


    <!-- http://w3.id.org/def/BibliOWL#isMemberOf -->


    <owl:ObjectProperty rdf:about="http://w3.id.org/def/BibliOWL#isMemberOf">
        <rdfs:subPropertyOf rdf:resource="http://www.w3.org/2002/07/owl#topObjectProperty"/>
        <rdfs:domain rdf:resource="http://datos.bne.es/def/C1005"/>
        <rdfs:range rdf:resource="http://datos.bne.es/def/C1006"/>
        <rdfs:label xml:lang="es">es miembro de</rdfs:label>
        <rdfs:label xml:lang="en">is member of</rdfs:label>
    </owl:ObjectProperty>
    


    <!-- http://w3.id.org/def/BibliOWL#isUserOf -->


    <owl:ObjectProperty rdf:about="http://w3.id.org/def/BibliOWL#isUserOf">
        <rdfs:domain rdf:resource="http://w3.id.org/def/BibliOWL#User"/>
        <rdfs:range rdf:resource="http://dati.beniculturali.it/cis/CulturalInstituteOrSite"/>
        <rdfs:isDefinedBy>http://w3.id.org/def/BibliOWL#</rdfs:isDefinedBy>
        <rdfs:label xml:lang="en">is user of</rdfs:label>
    </owl:ObjectProperty>
    


    <!-- http://w3.id.org/def/BibliOWL#participatesAtLoan -->


    <owl:ObjectProperty rdf:about="http://w3.id.org/def/BibliOWL#participatesAtLoan">
        <rdfs:domain rdf:resource="http://w3.id.org/def/BibliOWL#User"/>
        <rdfs:range rdf:resource="http://w3.id.org/def/BibliOWL#Loan"/>
        <rdfs:isDefinedBy>http://w3.id.org/def/BibliOWL#</rdfs:isDefinedBy>
        <rdfs:label xml:lang="en">(user) participates at Loan</rdfs:label>
    </owl:ObjectProperty>
    


    <!-- http://w3.id.org/def/BibliOWL#validDuring -->


    <owl:ObjectProperty rdf:about="http://w3.id.org/def/BibliOWL#validDuring">
        <rdfs:domain rdf:resource="http://w3.id.org/def/BibliOWL#Loan"/>
        <rdfs:range rdf:resource="http://dati.beniculturali.it/cis/TimeInterval"/>
        <rdfs:isDefinedBy>http://w3.id.org/def/BibliOWL#</rdfs:isDefinedBy>
        <rdfs:label xml:lang="en">valid during</rdfs:label>
    </owl:ObjectProperty>
    


    <!-- 
    ///////////////////////////////////////////////////////////////////////////////////////
    //
    // Data properties
    //
    ///////////////////////////////////////////////////////////////////////////////////////
     -->


    


    <!-- http://dati.beniculturali.it/cis/ISILIdentifier -->


    <owl:DatatypeProperty rdf:about="http://dati.beniculturali.it/cis/ISILIdentifier">
        <rdfs:subPropertyOf rdf:resource="http://dati.beniculturali.it/cis/identifier"/>
        <rdf:type rdf:resource="http://www.w3.org/2002/07/owl#FunctionalProperty"/>
        <rdfs:domain rdf:resource="http://dati.beniculturali.it/cis/CulturalInstituteOrSite"/>
        <rdfs:range rdf:resource="http://www.w3.org/2000/01/rdf-schema#Literal"/>
        <rdfs:comment xml:lang="it">Questa proprietà è utilizzata per rappresentare l&apos;identificativo univoco dell&apos;Istituto e luogo della cultura, i.e., il codice ISIL (International Standard identifier for Libraries and Related Organization). Sotto proprietà di identificativo.</rdfs:comment>
        <rdfs:comment xml:lang="en">This property is used to define the unique identifier of the cultural institute or site (i.e., the ISIL - International Standard Identifier for Libriaries and Related Organization - code). Subproperty of identifier.</rdfs:comment>
        <rdfs:isDefinedBy rdf:resource="http://dati.beniculturali.it/cis/"/>
        <rdfs:label xml:lang="en">ISIL identifier</rdfs:label>
        <rdfs:label xml:lang="it">Identificativo ISIL</rdfs:label>
        <owl:versionInfo xml:lang="it">Stabile</owl:versionInfo>
        <owl:versionInfo xml:lang="en">Stable</owl:versionInfo>
    </owl:DatatypeProperty>
    


    <!-- http://dati.beniculturali.it/cis/addressID -->


    <owl:DatatypeProperty rdf:about="http://dati.beniculturali.it/cis/addressID">
        <rdfs:subPropertyOf rdf:resource="http://dati.beniculturali.it/cis/identifier"/>
        <rdf:type rdf:resource="http://www.w3.org/2002/07/owl#FunctionalProperty"/>
        <rdfs:domain rdf:resource="http://dati.beniculturali.it/cis/Address"/>
        <rdfs:range rdf:resource="http://www.w3.org/2000/01/rdf-schema#Literal"/>
        <rdfs:comment xml:lang="en">Property used to represent the globally unique identifier for each instance of an address. A crucial part of the INSPIRE data specifications. Subproperty of identifier.</rdfs:comment>
        <rdfs:comment xml:lang="it">Proprietà utilizzata per rappresentare un identificatore univoco per ciascuna istanza di un indirizzo, Rappresenta un elemento cruciale delle specifiche INSPIRE. Sottoproprietà di identificativo.</rdfs:comment>
        <rdfs:isDefinedBy rdf:resource="http://dati.beniculturali.it/cis/"/>
        <rdfs:label xml:lang="en">address identifier</rdfs:label>
        <rdfs:label xml:lang="it">identificativo dell&apos;indirizzo</rdfs:label>
        <owl:versionInfo xml:lang="it">versione ancora non definitiva</owl:versionInfo>
        <owl:versionInfo>unstable</owl:versionInfo>
    </owl:DatatypeProperty>
    


    <!-- http://dati.beniculturali.it/cis/closes -->


    <owl:DatatypeProperty rdf:about="http://dati.beniculturali.it/cis/closes">
        <rdfs:domain rdf:resource="http://dati.beniculturali.it/cis/OpeningHoursSpecification"/>
        <rdfs:range rdf:resource="http://www.w3.org/2001/XMLSchema#time"/>
        <rdfs:comment xml:lang="it">Questa proprietà è utilizzata per rappresentare l&apos;orario di chiusura.</rdfs:comment>
        <rdfs:comment xml:lang="en">This property is used to represent the closing time</rdfs:comment>
        <rdfs:isDefinedBy rdf:resource="http://dati.beniculturali.it/cis/"/>
        <rdfs:label xml:lang="it">chiude </rdfs:label>
        <rdfs:label xml:lang="en">closes </rdfs:label>
        <owl:versionInfo xml:lang="it">stabile</owl:versionInfo>
        <owl:versionInfo xml:lang="en">stable</owl:versionInfo>
    </owl:DatatypeProperty>
    


    <!-- http://dati.beniculturali.it/cis/endDate -->


    <owl:DatatypeProperty rdf:about="http://dati.beniculturali.it/cis/endDate">
        <rdfs:domain rdf:resource="http://dati.beniculturali.it/cis/TimeInterval"/>
        <rdfs:range rdf:resource="http://www.w3.org/2001/XMLSchema#dateTime"/>
        <rdfs:comment xml:lang="it">Data di fine di un intervallo temporale</rdfs:comment>
        <rdfs:comment xml:lang="en">end Date of a Time Interval</rdfs:comment>
        <rdfs:isDefinedBy rdf:resource="http://dati.beniculturali.it/cis/"/>
        <rdfs:label xml:lang="it">data di fine</rdfs:label>
        <rdfs:label xml:lang="en">end Date</rdfs:label>
        <owl:versionInfo xml:lang="it">stabile</owl:versionInfo>
        <owl:versionInfo xml:lang="en">stable</owl:versionInfo>
    </owl:DatatypeProperty>
    


    <!-- http://dati.beniculturali.it/cis/fullAddress -->


    <owl:DatatypeProperty rdf:about="http://dati.beniculturali.it/cis/fullAddress">
        <rdfs:domain rdf:resource="http://dati.beniculturali.it/cis/Address"/>
        <rdfs:range rdf:resource="http://www.w3.org/2000/01/rdf-schema#Literal"/>
        <rdfs:comment xml:lang="en">Property used to represent the full address of the site of a cultural institute or site.</rdfs:comment>
        <rdfs:comment xml:lang="it">Proprietà utilizzata per indicare l&apos;indirizzo completo della sede di un istituto e luogo della cultura.</rdfs:comment>
        <rdfs:isDefinedBy rdf:resource="http://dati.beniculturali.it/cis/"/>
        <rdfs:label xml:lang="en">full address</rdfs:label>
        <rdfs:label xml:lang="it">indirizzo completo</rdfs:label>
        <owl:versionInfo xml:lang="it">stabile</owl:versionInfo>
        <owl:versionInfo>stable</owl:versionInfo>
    </owl:DatatypeProperty>
    


    <!-- http://dati.beniculturali.it/cis/hasEmail -->


    <owl:DatatypeProperty rdf:about="http://dati.beniculturali.it/cis/hasEmail">
        <rdfs:domain rdf:resource="http://dati.beniculturali.it/cis/ContactPoint"/>
        <rdfs:range rdf:resource="http://www.w3.org/2001/XMLSchema#anyURI"/>
        <rdfs:comment xml:lang="en">Property used to specify email address for a contact point</rdfs:comment>
        <rdfs:comment xml:lang="it">Proprietà utilizzata per specificare indirizzi email del punto di contatto</rdfs:comment>
        <rdfs:isDefinedBy rdf:resource="http://dati.beniculturali.it/cis/"/>
        <rdfs:label xml:lang="it">ha email</rdfs:label>
        <rdfs:label xml:lang="en">has email</rdfs:label>
        <owl:versionInfo xml:lang="it">stabile</owl:versionInfo>
        <owl:versionInfo xml:lang="en">stable</owl:versionInfo>
    </owl:DatatypeProperty>
    


    <!-- http://dati.beniculturali.it/cis/hasLat -->


    <owl:DatatypeProperty rdf:about="http://dati.beniculturali.it/cis/hasLat">
        <rdfs:domain rdf:resource="http://dati.beniculturali.it/cis/Geometry"/>
        <rdfs:range rdf:resource="http://www.w3.org/2001/XMLSchema#decimal"/>
        <rdfs:comment xml:lang="en">Property used to associate a latitude with a Point</rdfs:comment>
        <rdfs:comment xml:lang="it">Proprietà utilizzata per associare la latitudine a un punto</rdfs:comment>
        <rdfs:isDefinedBy rdf:resource="http://dati.beniculturali.it/cis/"/>
        <rdfs:label xml:lang="it">ha latitudine</rdfs:label>
        <rdfs:label xml:lang="en">has latitude</rdfs:label>
        <owl:versionInfo xml:lang="it">stabile</owl:versionInfo>
        <owl:versionInfo>stable</owl:versionInfo>
    </owl:DatatypeProperty>
    


    <!-- http://dati.beniculturali.it/cis/hasLong -->


    <owl:DatatypeProperty rdf:about="http://dati.beniculturali.it/cis/hasLong">
        <rdfs:domain rdf:resource="http://dati.beniculturali.it/cis/Geometry"/>
        <rdfs:range rdf:resource="http://www.w3.org/2001/XMLSchema#decimal"/>
        <rdfs:comment xml:lang="en">Property used to associate the longitude with a Point</rdfs:comment>
        <rdfs:comment xml:lang="it">Proprietà utilizzata per associare la longitudine a un punto</rdfs:comment>
        <rdfs:isDefinedBy rdf:resource="http://dati.beniculturali.it/cis/"/>
        <rdfs:label xml:lang="it">ha longitudine</rdfs:label>
        <rdfs:label xml:lang="en">has longitude</rdfs:label>
        <owl:versionInfo xml:lang="it">stabile</owl:versionInfo>
        <owl:versionInfo>stable</owl:versionInfo>
    </owl:DatatypeProperty>
    


    <!-- http://dati.beniculturali.it/cis/hasReason -->


    <owl:DatatypeProperty rdf:about="http://dati.beniculturali.it/cis/hasReason">
        <rdfs:domain rdf:resource="http://dati.beniculturali.it/cis/TemporaryClosure"/>
        <rdfs:range rdf:resource="http://www.w3.org/2000/01/rdf-schema#Literal"/>
        <rdfs:comment xml:lang="en">Property used to describe a reason for the temporary closure.</rdfs:comment>
        <rdfs:comment xml:lang="it">Proprietà utilizzata per descrivere una motivazione della chiusura temporanea.</rdfs:comment>
        <rdfs:isDefinedBy rdf:resource="http://dati.beniculturali.it/cis/"/>
        <rdfs:label xml:lang="it">ha motivazione</rdfs:label>
        <rdfs:label xml:lang="en">has reason</rdfs:label>
        <owl:versionInfo xml:lang="it">stabile</owl:versionInfo>
        <owl:versionInfo>stable</owl:versionInfo>
    </owl:DatatypeProperty>
    


    <!-- http://dati.beniculturali.it/cis/hasTelephone -->


    <owl:DatatypeProperty rdf:about="http://dati.beniculturali.it/cis/hasTelephone">
        <rdfs:domain rdf:resource="http://dati.beniculturali.it/cis/ContactPoint"/>
        <rdfs:range rdf:resource="http://www.w3.org/2000/01/rdf-schema#Literal"/>
        <rdfs:comment xml:lang="en">Property used to represent one or more telephone numbers for the contact point</rdfs:comment>
        <rdfs:comment xml:lang="it">proprietà utilizzata per rappresentare uno o più numeri di telefono per il punto di contatto</rdfs:comment>
        <rdfs:isDefinedBy rdf:resource="http://dati.beniculturali.it/cis/"/>
        <rdfs:label xml:lang="it">ha telefono</rdfs:label>
        <rdfs:label xml:lang="en">has telephone</rdfs:label>
        <owl:versionInfo xml:lang="it">stabile</owl:versionInfo>
        <owl:versionInfo xml:lang="en">stable</owl:versionInfo>
    </owl:DatatypeProperty>
    


    <!-- http://dati.beniculturali.it/cis/hasWebSite -->


    <owl:DatatypeProperty rdf:about="http://dati.beniculturali.it/cis/hasWebSite">
        <rdfs:domain rdf:resource="http://dati.beniculturali.it/cis/CulturalInstituteOrSite"/>
        <rdfs:range rdf:resource="http://www.w3.org/2001/XMLSchema#anyURI"/>
        <rdfs:comment xml:lang="en">Property used to represent a web site</rdfs:comment>
        <rdfs:comment xml:lang="it">Proprietà utilizzata per rappresentare un sito web</rdfs:comment>
        <rdfs:isDefinedBy rdf:resource="http://dati.beniculturali.it/cis/"/>
        <rdfs:label xml:lang="it">ha sito web</rdfs:label>
        <rdfs:label xml:lang="en">has web site</rdfs:label>
        <owl:versionInfo xml:lang="it">stabile</owl:versionInfo>
        <owl:versionInfo xml:lang="en">stable</owl:versionInfo>
    </owl:DatatypeProperty>
    


    <!-- http://dati.beniculturali.it/cis/identifier -->


    <owl:DatatypeProperty rdf:about="http://dati.beniculturali.it/cis/identifier">
        <rdf:type rdf:resource="http://www.w3.org/2002/07/owl#FunctionalProperty"/>
        <rdfs:domain rdf:resource="http://www.w3.org/2002/07/owl#Thing"/>
        <rdfs:range rdf:resource="http://www.w3.org/2000/01/rdf-schema#Literal"/>
        <rdfs:comment xml:lang="it">Questa proprietà rappresenta un identificativo per una cosa.</rdfs:comment>
        <rdfs:comment xml:lang="en">This property represents an identifier for a Thing.</rdfs:comment>
        <rdfs:isDefinedBy rdf:resource="http://dati.beniculturali.it/cis/"/>
        <rdfs:label xml:lang="it">identificativo</rdfs:label>
        <rdfs:label xml:lang="en">identifier</rdfs:label>
        <owl:versionInfo xml:lang="it">stabile</owl:versionInfo>
        <owl:versionInfo xml:lang="en">stable</owl:versionInfo>
    </owl:DatatypeProperty>
    


    <!-- http://dati.beniculturali.it/cis/institutionalName -->


    <owl:DatatypeProperty rdf:about="http://dati.beniculturali.it/cis/institutionalName">
        <rdfs:subPropertyOf rdf:resource="http://dati.beniculturali.it/cis/name"/>
        <rdfs:domain rdf:resource="http://dati.beniculturali.it/cis/CulturalInstituteOrSite"/>
        <rdfs:range rdf:resource="http://www.w3.org/2000/01/rdf-schema#Literal"/>
        <rdfs:comment xml:lang="it">Questa proprietà identifica direttamente il nome istituzionale dell&apos;Istituto e luogo della cultura</rdfs:comment>
        <rdfs:comment xml:lang="en">This data property identifies  the institutional name of the Cultural Institute or Site.</rdfs:comment>
        <rdfs:isDefinedBy rdf:resource="http://dati.beniculturali.it/cis/"/>
        <rdfs:label xml:lang="it">Nome Istituzionale</rdfs:label>
        <rdfs:label>Institutional Name</rdfs:label>
        <owl:versionInfo xml:lang="it">Stabile</owl:versionInfo>
        <owl:versionInfo xml:lang="en">Stable</owl:versionInfo>
    </owl:DatatypeProperty>
    


    <!-- http://dati.beniculturali.it/cis/name -->


    <owl:DatatypeProperty rdf:about="http://dati.beniculturali.it/cis/name">
        <rdfs:domain rdf:resource="http://www.w3.org/2002/07/owl#Thing"/>
        <rdfs:range rdf:resource="http://www.w3.org/2000/01/rdf-schema#Literal"/>
        <rdfs:comment xml:lang="en">Property used to associate a name with an event and a project</rdfs:comment>
        <rdfs:comment xml:lang="it">Proprietà utilizzata per associare un nome all&apos;evento o al progetto</rdfs:comment>
        <rdfs:isDefinedBy rdf:resource="http://dati.beniculturali.it/cis/"/>
        <rdfs:label xml:lang="en">name</rdfs:label>
        <rdfs:label xml:lang="it">nome</rdfs:label>
        <owl:versionInfo xml:lang="it">stabile</owl:versionInfo>
        <owl:versionInfo>stable</owl:versionInfo>
    </owl:DatatypeProperty>
    


    <!-- http://dati.beniculturali.it/cis/opens -->


    <owl:DatatypeProperty rdf:about="http://dati.beniculturali.it/cis/opens">
        <rdfs:domain rdf:resource="http://dati.beniculturali.it/cis/OpeningHoursSpecification"/>
        <rdfs:range rdf:resource="http://www.w3.org/2001/XMLSchema#time"/>
        <rdfs:comment xml:lang="it">Questa proprietà è utilizzata per rappresentare l&apos;orario di apertura</rdfs:comment>
        <rdfs:comment xml:lang="en">This property is used to represent the opening time</rdfs:comment>
        <rdfs:isDefinedBy rdf:resource="http://dati.beniculturali.it/cis/"/>
        <rdfs:label xml:lang="it">apre </rdfs:label>
        <rdfs:label xml:lang="en">opens </rdfs:label>
        <owl:versionInfo xml:lang="it">non stabile</owl:versionInfo>
        <owl:versionInfo xml:lang="en">unstable</owl:versionInfo>
    </owl:DatatypeProperty>
    


    <!-- http://dati.beniculturali.it/cis/postCode -->


    <owl:DatatypeProperty rdf:about="http://dati.beniculturali.it/cis/postCode">
        <rdfs:domain rdf:resource="http://dati.beniculturali.it/cis/Address"/>
        <rdfs:range rdf:resource="http://www.w3.org/2000/01/rdf-schema#Literal"/>
        <rdfs:comment xml:lang="en">Property used to represent the post code of the address of the site of a cultural institute or site.</rdfs:comment>
        <rdfs:comment xml:lang="it">Proprietà utilizzata per rappresentare il codice postale.</rdfs:comment>
        <rdfs:isDefinedBy rdf:resource="http://dati.beniculturali.it/cis/"/>
        <rdfs:label xml:lang="it">codice postale</rdfs:label>
        <rdfs:label xml:lang="en">post code</rdfs:label>
        <owl:versionInfo xml:lang="it">stabile</owl:versionInfo>
        <owl:versionInfo>stable</owl:versionInfo>
    </owl:DatatypeProperty>
    


    <!-- http://dati.beniculturali.it/cis/startDate -->


    <owl:DatatypeProperty rdf:about="http://dati.beniculturali.it/cis/startDate">
        <rdfs:domain rdf:resource="http://dati.beniculturali.it/cis/TimeInterval"/>
        <rdfs:range rdf:resource="http://www.w3.org/2001/XMLSchema#dateTime"/>
        <rdfs:comment xml:lang="it">Data di inizio di un intervella temporale</rdfs:comment>
        <rdfs:comment xml:lang="en">Srart date of a Time Interval</rdfs:comment>
        <rdfs:isDefinedBy rdf:resource="http://dati.beniculturali.it/cis/"/>
        <rdfs:label xml:lang="it">Data di inizio</rdfs:label>
        <rdfs:label xml:lang="en">start Date</rdfs:label>
        <owl:versionInfo xml:lang="it">stabile</owl:versionInfo>
        <owl:versionInfo xml:lang="en">stable</owl:versionInfo>
    </owl:DatatypeProperty>
    


    <!-- http://dati.beniculturali.it/cis/toponym -->


    <owl:DatatypeProperty rdf:about="http://dati.beniculturali.it/cis/toponym">
        <rdfs:subPropertyOf rdf:resource="http://dati.beniculturali.it/cis/name"/>
        <rdfs:domain rdf:resource="http://dati.beniculturali.it/cis/GeographicalFeature"/>
        <rdfs:range rdf:resource="http://www.w3.org/2000/01/rdf-schema#Literal"/>
        <rdfs:comment xml:lang="it">Proprietà che rappresenta il toponimo dell&apos;area geografica.</rdfs:comment>
        <rdfs:comment xml:lang="en">This property represents the toponym of a geographical area.</rdfs:comment>
        <rdfs:label xml:lang="it">toponimo</rdfs:label>
        <rdfs:label xml:lang="en">toponym</rdfs:label>
        <owl:versionInfo xml:lang="it">stabile</owl:versionInfo>
        <owl:versionInfo xml:lang="en">stable</owl:versionInfo>
    </owl:DatatypeProperty>
    


    <!-- http://datos.bne.es/def/P1001 -->


    <owl:DatatypeProperty rdf:about="http://datos.bne.es/def/P1001">
        <rdfs:subPropertyOf rdf:resource="http://dati.beniculturali.it/cis/name"/>
        <rdfs:domain rdf:resource="http://datos.bne.es/def/C1001"/>
        <rdfs:range rdf:resource="http://www.w3.org/2000/01/rdf-schema#Literal"/>
        <rdfs:label xml:lang="en">has title of the work</rdfs:label>
    </owl:DatatypeProperty>
    


    <!-- http://datos.bne.es/def/P1004 -->


    <owl:DatatypeProperty rdf:about="http://datos.bne.es/def/P1004">
        <rdfs:domain rdf:resource="http://datos.bne.es/def/C1001"/>
        <rdfs:range rdf:resource="http://www.w3.org/2001/XMLSchema#date"/>
        <rdfs:label xml:lang="en">has date of the work</rdfs:label>
    </owl:DatatypeProperty>
    


    <!-- http://datos.bne.es/def/P1008 -->


    <owl:DatatypeProperty rdf:about="http://datos.bne.es/def/P1008">
        <rdfs:domain rdf:resource="http://w3.id.org/def/BibliOWL#Music"/>
        <rdfs:range rdf:resource="http://www.w3.org/2000/01/rdf-schema#Literal"/>
        <rdfs:label xml:lang="en">has medium of performance (musical work)</rdfs:label>
    </owl:DatatypeProperty>
    


    <!-- http://datos.bne.es/def/P2001 -->


    <owl:DatatypeProperty rdf:about="http://datos.bne.es/def/P2001">
        <rdfs:domain rdf:resource="http://datos.bne.es/def/C1002"/>
        <rdfs:range rdf:resource="http://www.w3.org/2000/01/rdf-schema#Literal"/>
        <rdfs:label xml:lang="en">has language of expression</rdfs:label>
    </owl:DatatypeProperty>
    


    <!-- http://datos.bne.es/def/P3004 -->


    <owl:DatatypeProperty rdf:about="http://datos.bne.es/def/P3004">
        <rdfs:domain rdf:resource="http://datos.bne.es/def/C1003"/>
        <rdfs:range rdf:resource="http://www.w3.org/2000/01/rdf-schema#Literal"/>
        <rdfs:label xml:lang="en">has specific material designation and extent</rdfs:label>
    </owl:DatatypeProperty>
    


    <!-- http://datos.bne.es/def/P3013 -->


    <owl:DatatypeProperty rdf:about="http://datos.bne.es/def/P3013">
        <rdfs:subPropertyOf rdf:resource="http://dati.beniculturali.it/cis/identifier"/>
        <rdfs:domain rdf:resource="http://datos.bne.es/def/C1003"/>
        <rdfs:range rdf:resource="http://www.w3.org/2000/01/rdf-schema#Literal"/>
        <rdfs:label xml:lang="en">ISBN</rdfs:label>
    </owl:DatatypeProperty>
    


    <!-- http://datos.bne.es/def/P3015 -->


    <owl:DatatypeProperty rdf:about="http://datos.bne.es/def/P3015">
        <rdfs:domain rdf:resource="http://datos.bne.es/def/C1003"/>
        <rdfs:range rdf:resource="http://www.w3.org/2000/01/rdf-schema#Literal"/>
        <rdfs:label xml:lang="en">has note</rdfs:label>
    </owl:DatatypeProperty>
    


    <!-- http://datos.bne.es/def/P3048 -->


    <owl:DatatypeProperty rdf:about="http://datos.bne.es/def/P3048">
        <rdfs:domain rdf:resource="http://datos.bne.es/def/C1003"/>
        <rdfs:range rdf:resource="http://www.w3.org/2001/XMLSchema#date"/>
        <rdfs:label xml:lang="en">has date of printing or manufacturer</rdfs:label>
    </owl:DatatypeProperty>
    


    <!-- http://datos.bne.es/def/P5001 -->


    <owl:DatatypeProperty rdf:about="http://datos.bne.es/def/P5001">
        <rdfs:subPropertyOf rdf:resource="http://dati.beniculturali.it/cis/name"/>
        <rdfs:domain rdf:resource="http://datos.bne.es/def/C1005"/>
        <rdfs:range rdf:resource="http://www.w3.org/2000/01/rdf-schema#Literal"/>
        <rdfs:label xml:lang="en">has name of person</rdfs:label>
    </owl:DatatypeProperty>
    


    <!-- http://datos.bne.es/def/P5005 -->


    <owl:DatatypeProperty rdf:about="http://datos.bne.es/def/P5005">
        <rdfs:domain rdf:resource="http://datos.bne.es/def/C1005"/>
        <rdfs:range>
            <rdfs:Datatype>
                <owl:unionOf rdf:parseType="Collection">
                    <rdf:Description rdf:about="http://www.w3.org/2000/01/rdf-schema#Literal"/>
                    <rdf:Description rdf:about="http://www.w3.org/2001/XMLSchema#anyURI"/>
                </owl:unionOf>
            </rdfs:Datatype>
        </rdfs:range>
        <rdfs:label xml:lang="en">has biography or history</rdfs:label>
    </owl:DatatypeProperty>
    


    <!-- http://datos.bne.es/def/P5008 -->


    <owl:DatatypeProperty rdf:about="http://datos.bne.es/def/P5008">
        <rdfs:domain rdf:resource="http://datos.bne.es/def/C1005"/>
        <rdfs:range rdf:resource="http://www.w3.org/2000/01/rdf-schema#Literal"/>
        <rdfs:label xml:lang="en">has pseudonymous</rdfs:label>
    </owl:DatatypeProperty>
    


    <!-- http://datos.bne.es/def/P5010 -->


    <owl:DatatypeProperty rdf:about="http://datos.bne.es/def/P5010">
        <rdfs:domain rdf:resource="http://datos.bne.es/def/C1005"/>
        <rdfs:range rdf:resource="http://www.w3.org/2001/XMLSchema#date"/>
        <rdfs:label xml:lang="en">date of birth</rdfs:label>
    </owl:DatatypeProperty>
    


    <!-- http://datos.bne.es/def/P5011 -->


    <owl:DatatypeProperty rdf:about="http://datos.bne.es/def/P5011">
        <rdfs:domain rdf:resource="http://datos.bne.es/def/C1005"/>
        <rdfs:range rdf:resource="http://www.w3.org/2001/XMLSchema#date"/>
        <rdfs:label xml:lang="en">date of death</rdfs:label>
    </owl:DatatypeProperty>
    


    <!-- http://w3.id.org/def/BibliOWL#corporateBodyName -->


    <owl:DatatypeProperty rdf:about="http://w3.id.org/def/BibliOWL#corporateBodyName">
        <rdfs:subPropertyOf rdf:resource="http://dati.beniculturali.it/cis/name"/>
        <rdfs:domain rdf:resource="http://datos.bne.es/def/C1006"/>
        <rdfs:range rdf:resource="http://www.w3.org/2000/01/rdf-schema#Literal"/>
        <rdfs:isDefinedBy>http://w3.id.org/def/BibliOWL#</rdfs:isDefinedBy>
        <rdfs:label xml:lang="en">has Corporate Body name</rdfs:label>
    </owl:DatatypeProperty>
    


    <!-- http://w3.id.org/def/BibliOWL#hasAppropiateAge -->


    <owl:DatatypeProperty rdf:about="http://w3.id.org/def/BibliOWL#hasAppropiateAge">
        <rdfs:domain rdf:resource="http://datos.bne.es/def/C1003"/>
        <rdfs:range rdf:resource="http://www.w3.org/2001/XMLSchema#int"/>
        <rdfs:isDefinedBy>http://w3.id.org/def/BibliOWL#</rdfs:isDefinedBy>
        <rdfs:label xml:lang="en">has appropiate age</rdfs:label>
    </owl:DatatypeProperty>
    


    <!-- http://w3.id.org/def/BibliOWL#hasGenre -->


    <owl:DatatypeProperty rdf:about="http://w3.id.org/def/BibliOWL#hasGenre">
        <rdfs:domain rdf:resource="http://datos.bne.es/def/C1001"/>
        <rdfs:range rdf:resource="http://www.w3.org/2000/01/rdf-schema#Literal"/>
        <rdfs:isDefinedBy>http://w3.id.org/def/BibliOWL#</rdfs:isDefinedBy>
        <rdfs:label xml:lang="en">has genre</rdfs:label>
    </owl:DatatypeProperty>
    


    <!-- http://w3.id.org/def/BibliOWL#itemID -->


    <owl:DatatypeProperty rdf:about="http://w3.id.org/def/BibliOWL#itemID">
        <rdfs:subPropertyOf rdf:resource="http://dati.beniculturali.it/cis/identifier"/>
        <rdfs:domain rdf:resource="http://datos.bne.es/def/C1004"/>
        <rdfs:range rdf:resource="http://www.w3.org/2000/01/rdf-schema#Literal"/>
        <rdfs:label xml:lang="es">ejemplar ID</rdfs:label>
        <rdfs:label xml:lang="en">item ID</rdfs:label>
    </owl:DatatypeProperty>
    


    <!-- http://w3.id.org/def/BibliOWL#loanID -->


    <owl:DatatypeProperty rdf:about="http://w3.id.org/def/BibliOWL#loanID">
        <rdfs:subPropertyOf rdf:resource="http://dati.beniculturali.it/cis/identifier"/>
        <rdfs:domain rdf:resource="http://w3.id.org/def/BibliOWL#Loan"/>
        <rdfs:range rdf:resource="http://www.w3.org/2000/01/rdf-schema#Literal"/>
        <rdfs:isDefinedBy>http://w3.id.org/def/BibliOWL#</rdfs:isDefinedBy>
        <rdfs:label xml:lang="en">Loan ID</rdfs:label>
    </owl:DatatypeProperty>
    


    <!-- http://w3.id.org/def/BibliOWL#userID -->


    <owl:DatatypeProperty rdf:about="http://w3.id.org/def/BibliOWL#userID">
        <rdfs:subPropertyOf rdf:resource="http://dati.beniculturali.it/cis/identifier"/>
        <rdfs:domain rdf:resource="http://w3.id.org/def/BibliOWL#User"/>
        <rdfs:range rdf:resource="http://www.w3.org/2000/01/rdf-schema#Literal"/>
        <rdfs:isDefinedBy xml:lang="en">http://w3.id.org/def/BibliOWL#</rdfs:isDefinedBy>
        <rdfs:label xml:lang="en">user ID</rdfs:label>
    </owl:DatatypeProperty>
    


    <!-- 
    ///////////////////////////////////////////////////////////////////////////////////////
    //
    // Classes
    //
    ///////////////////////////////////////////////////////////////////////////////////////
     -->


    


    <!-- http://dati.beniculturali.it/cis/AccessCondition -->


    <owl:Class rdf:about="http://dati.beniculturali.it/cis/AccessCondition">
        <dc:description rdf:resource="http://dati.beniculturali.it/cis/img/access.png"/>
        <dc:description xml:lang="it">Questa classe è utilizzata per rappresentare le condizioni di accesso associate a un &quot;Istituto e luogo della Culrura&quot; o a un &quot;Evento&quot;: Le condizione di accesso sono individui delle seguenti classi:
 * Orari di apertura
 * Chiusara Temporanea
 * Tipo di Prenotazione

Un esempio dell&apos;uso della classe in turle è il seguente:
&lt;pre&gt;
cis a CulturalInstituteOrSite ;
  description &quot;An entity representing an individual of the class &apos;Institute or Site.&apos;&quot; ;
  hasAccessCondition cis_access_condition . 

cis_access_condition a Access ;
  description &quot;The individual of the class &apos;Access&apos; that specifies the access
  condition associated with the CulturalInstituteOrSite called cis&quot; .
&lt;/pre&gt;</dc:description>
        <dc:description xml:lang="en">This class is used for representing the access conditions associated with a &apos;Cultural Institute or Site&apos; or an &apos;Event&apos;.
Access conditions are meant to be indivuduals of the following classes:
  * Opening Hours Specification
  * Temporary Closure
  * Type of Booking

An example in turtle is the following:

&lt;pre&gt;
cis a CulturalInstituteOrSite ;
  description &quot;An entity representing an individual of the class &apos;Institute or Site.&apos;&quot; ;
  hasAccessCondition cis_access_condition . 

cis_access_condition a Access ;
  description &quot;The individual of the class &apos;Access&apos; that specifies the access
  condition associated with the CulturalInstituteOrSite called cis&quot; .
&lt;/pre&gt;</dc:description>
        <rdfs:comment xml:lang="en">Concept used to represent general information for the public access to the Cultural Institute or Site or to the Event. For instance, examples of information include: opening hours, type of admission, temporary closing, etc.</rdfs:comment>
        <rdfs:comment xml:lang="it">Concetto che rappresenta le informazioni generali per l&apos;accesso da parte del pubblico all&apos;Istituto e Luogo della Cultura e all&apos;evento. Per esempio consente di modellare informazioni quali gi orari di apertura, le chiusure temporanee (con le relative motivazioni), il tipo di apertura al pubblico, ecc.</rdfs:comment>
        <rdfs:isDefinedBy rdf:resource="http://dati.beniculturali.it/cis/"/>
        <rdfs:label xml:lang="en">Access condition</rdfs:label>
        <rdfs:label xml:lang="it">Condizioni di accesso</rdfs:label>
        <owl:versionInfo xml:lang="it">stabile</owl:versionInfo>
        <owl:versionInfo xml:lang="en">stable</owl:versionInfo>
    </owl:Class>
    


    <!-- http://dati.beniculturali.it/cis/Address -->


    <owl:Class rdf:about="http://dati.beniculturali.it/cis/Address">
        <rdfs:subClassOf>
            <owl:Restriction>
                <owl:onProperty rdf:resource="http://dati.beniculturali.it/cis/fullAddress"/>
                <owl:someValuesFrom rdf:resource="http://www.w3.org/2000/01/rdf-schema#Literal"/>
            </owl:Restriction>
        </rdfs:subClassOf>
        <rdfs:subClassOf>
            <owl:Restriction>
                <owl:onProperty rdf:resource="http://dati.beniculturali.it/cis/postCode"/>
                <owl:someValuesFrom rdf:resource="http://www.w3.org/2000/01/rdf-schema#Literal"/>
            </owl:Restriction>
        </rdfs:subClassOf>
        <rdfs:subClassOf>
            <owl:Restriction>
                <owl:onProperty rdf:resource="http://dati.beniculturali.it/cis/addressID"/>
                <owl:cardinality rdf:datatype="http://www.w3.org/2001/XMLSchema#nonNegativeInteger">1</owl:cardinality>
            </owl:Restriction>
        </rdfs:subClassOf>
        <dc:description rdf:resource="http://dati.beniculturali.it/cis/img/address.png"/>
        <dc:description xml:lang="en">Individuals of the class Site are associated with individual of the class Address by means of the object property hasAddress.
An address is characterised by the following properties:

 * addressIdentifier: a unique ID of the address;
 * administrativeUnitLevel1: e.g., Rome;
 * administrativeUnitLevel2: e.g., Lazio;
 * fullAddress: the literal that records the full address as a string;
 * postCode: the postal code corresponding to the address;
 * postName: the key postal name, usually the city ;


An example in turtle is the following:

&lt;pre&gt;

site:Sede_di_Biblioteca_nazionale_centrale_di_Roma
      a       cis:Site ;
      rdfs:label &quot;Sede di: Biblioteca nazionale centrale di Roma&quot;@it ;
      cis:hasAddress address:Indirizzo_della_sede_di_Biblioteca_nazionale_centrale_di_Roma ;


address:Indirizzo_della_sede_di_Biblioteca_nazionale_centrale_di_Roma
      a       cis:Address ;
      rdfs:label &quot;Indirizzo della sede di: Biblioteca nazionale centrale di Roma&quot;@it ;
      cis:addressID &quot;IT-RM0267_IT_1&quot; ;
      cis:adminUnitL1 &quot;Roma&quot;@it ;
      cis:adminUnitL2 &quot;Lazio&quot;@it ;
      cis:fullAddress &quot;Viale Castro Pretorio 105 - 00185 - Roma (RM&quot; ;
      cis:postName &quot;Rome&quot; ;
      cis:postCode &quot;00185&quot; .

&lt;/pre&gt;</dc:description>
        <dc:description xml:lang="it">Individui della classe Address sono connessi ad invididui della classe Site attraverso la proprietà che collega Site ad Address hasAddress. 
Un indirizzo è caratterizzato dalle seguenti proprietà:

 * Identificativo dell&apos;indirizzo: un ID univoco dell&apos;indirizzo;
 * livello amministrativo 1: di solito il comune, e.g., Roma;
 * livello amministrativo 2: di solito la regione, e.g., Lazio;
 * indirizzo completo: un literal che rappresenta l&apos;indirizzo completo come una stringa
 * codice postale: il codice postale corrispondere all&apos;indirizzo.
 * nome postale: il nome chiave postale di solito la città

Un esempio in turtle è il seguente:
site:Sede_di_Biblioteca_nazionale_centrale_di_Roma
      a       cis:Site ;
      rdfs:label &quot;Sede di: Biblioteca nazionale centrale di Roma&quot;@it ;
      cis:hasAddress address:Indirizzo_della_sede_di_Biblioteca_nazionale_centrale_di_Roma ;


address:Indirizzo_della_sede_di_Biblioteca_nazionale_centrale_di_Roma
      a       cis:Address ;
      rdfs:label &quot;Indirizzo della sede di: Biblioteca nazionale centrale di Roma&quot;@it ;
      cis:addressID &quot;IT-RM0267_IT_1&quot; ;
      cis:adminUnitL1 &quot;Roma&quot;@it ;
      cis:adminUnitL2 &quot;Lazio&quot;@it ;
      cis:fullAddress &quot;Viale Castro Pretorio 105 - 00185 - Roma (RM&quot;) ;
      cis:postName &quot;Roma&quot; ;
      cis:postCode &quot;00185&quot; .

&lt;/pre&gt;</dc:description>
        <rdfs:comment xml:lang="en">It represents an address as defined by the specifications of the EU INSPIRE directive https://inspire-twg.jrc.ec.europa.eu/inspire-fc.html#_C2538</rdfs:comment>
        <rdfs:comment xml:lang="it">Rappresenta un indirizzo così come descritto nelle specifiche della direttiva Europea INSPIRE https://inspire-twg.jrc.ec.europa.eu/inspire-fc.html#_C2538.</rdfs:comment>
        <rdfs:isDefinedBy rdf:resource="http://dati.beniculturali.it/cis/"/>
        <rdfs:label xml:lang="en">Address</rdfs:label>
        <rdfs:label xml:lang="it">Indirizzo</rdfs:label>
        <owl:versionInfo xml:lang="it">stabile</owl:versionInfo>
        <owl:versionInfo xml:lang="en">stable</owl:versionInfo>
    </owl:Class>
    


    <!-- http://dati.beniculturali.it/cis/Catalogue -->


    <owl:Class rdf:about="http://dati.beniculturali.it/cis/Catalogue">
        <rdfs:subClassOf>
            <owl:Restriction>
                <owl:onProperty rdf:resource="http://dati.beniculturali.it/cis/isCatalogueOf"/>
                <owl:allValuesFrom rdf:resource="http://dati.beniculturali.it/cis/CulturalInstituteOrSite"/>
            </owl:Restriction>
        </rdfs:subClassOf>
        <rdfs:subClassOf>
            <owl:Restriction>
                <owl:onProperty rdf:resource="http://dati.beniculturali.it/cis/name"/>
                <owl:someValuesFrom rdf:resource="http://www.w3.org/2000/01/rdf-schema#Literal"/>
            </owl:Restriction>
        </rdfs:subClassOf>
        <rdfs:subClassOf>
            <owl:Restriction>
                <owl:onProperty rdf:resource="http://dati.beniculturali.it/cis/hasWebSite"/>
                <owl:allValuesFrom rdf:resource="http://www.w3.org/2001/XMLSchema#anyURI"/>
            </owl:Restriction>
        </rdfs:subClassOf>
        <dc:description rdf:resource="http://dati.beniculturali.it/cis/img/catalogue.png"/>
        <dc:description xml:lang="en">A catalogue is always associated with an individual of the class &apos;CulturalInstituteOrSite&apos; (CIS) by means of the object property hasCatalogue (with domain CulturalInstituteOrSite and range Catalogue).

The inverse property of hasCatalogue is isCatalogueOf and relates a catalogue to a CIS.

An example in turtle is the following:

&lt;pre&gt;
catalogue:Catalogo_Generale_(autore)
      a       cis:Catalogue ;
      rdfs:label &quot;Catalogo Generale (autore)&quot; ;
      cis:name &quot;Catalogo Generale (autore)&quot; ;
      cis:isCatalogueOf cissite:Biblioteca_nazionale_centrale ;
      cis:description &quot;Catalogo Generale per autore - online&quot;@it .

cissite:Biblioteca_nazionale_centrale
      a       cis:Library , cis:CulturalInstituteOrSite ;
      cis:hasCatalogue catalogue:Catalogo_Generale_(autore) .
&lt;/pre&gt;</dc:description>
        <dc:description xml:lang="it">Un catalogo è sempre associato a un individuo della classe &quot;Istitute e luogo della cultura&quot; attraverso la proprietà ha catalogo (che ha dominio CulturaInstituteOrSite e codominio Catalogue).

La proprietà inversa di ha catalogo è &quot;è catalogo di&quot; e collega il catalogo all&apos;istituto e luogo della cultura.

Un esempio in turtle è il seguente:

&lt;pre&gt;

catalogue:Catalogo_Generale_(autore)
      a       cis:Catalogue ;
      rdfs:label &quot;Catalogo Generale (autore)&quot; ;
      cis:name &quot;Catalogo Generale (autore)&quot; ;
      cis:isCatalogueOf cissite:Biblioteca_nazionale_centrale ;
      cis:description &quot;Catalogo Generale per autore - online&quot;@it .

cissite:Biblioteca_nazionale_centrale
      a       cis:Library , cis:CulturalInstituteOrSite ;
      cis:hasCatalogue catalogue:Catalogo_Generale_(autore) .

&lt;/pre&gt;</dc:description>
        <rdfs:comment xml:lang="en">Concept used to represent the catalogue which describes the set of cultural heritage objects included in a Cultural Institute or Site</rdfs:comment>
        <rdfs:comment xml:lang="it">Concetto utilizzato per rappresentare il catalogo che descrive l&apos;insieme delle opere contenute in un istituto e luogo della cultura.</rdfs:comment>
        <rdfs:isDefinedBy rdf:resource="http://dati.beniculturali.it/cis/"/>
        <rdfs:label xml:lang="it">Catalogo</rdfs:label>
        <rdfs:label xml:lang="en">Catalogue</rdfs:label>
        <owl:versionInfo xml:lang="it">stabile</owl:versionInfo>
        <owl:versionInfo xml:lang="en">stable</owl:versionInfo>
    </owl:Class>
    


    <!-- http://dati.beniculturali.it/cis/ContactPoint -->


    <owl:Class rdf:about="http://dati.beniculturali.it/cis/ContactPoint">
        <rdfs:subClassOf>
            <owl:Restriction>
                <owl:onProperty rdf:resource="http://dati.beniculturali.it/cis/available"/>
                <owl:allValuesFrom rdf:resource="http://dati.beniculturali.it/cis/OpeningHoursSpecification"/>
            </owl:Restriction>
        </rdfs:subClassOf>
        <rdfs:subClassOf>
            <owl:Restriction>
                <owl:onProperty rdf:resource="http://dati.beniculturali.it/cis/hasEmail"/>
                <owl:allValuesFrom rdf:resource="http://www.w3.org/2001/XMLSchema#anyURI"/>
            </owl:Restriction>
        </rdfs:subClassOf>
        <rdfs:subClassOf>
            <owl:Restriction>
                <owl:onProperty rdf:resource="http://dati.beniculturali.it/cis/hasTelephone"/>
                <owl:allValuesFrom rdf:resource="http://www.w3.org/2001/XMLSchema#anyURI"/>
            </owl:Restriction>
        </rdfs:subClassOf>
        <rdfs:subClassOf>
            <owl:Restriction>
                <owl:onProperty rdf:resource="http://dati.beniculturali.it/cis/hasWebSite"/>
                <owl:allValuesFrom rdf:resource="http://www.w3.org/2001/XMLSchema#anyURI"/>
            </owl:Restriction>
        </rdfs:subClassOf>
        <dc:description xml:lang="it">Gli individui delle classi Istituto e Luogo della Cultura, Evento e Sede possono avere dei punti di contatto, i.e., un numero di telefono, un indirizzo email, un fax, ecc. che sono utilizzati come riferimenti.

Inoltre, un pubto di contatto potrebbe essere dichiarato come operativo in alcune fasce orarie.

Queste informazioni sono modellate attraverso l&apos;uso della proprietà ha punto di contatto il cui dominio può essere un Istituto e Luogo della Cultura, un Evento o una Sede e il suo range qualsiasi individuo della classe Punto di Contatto.

Per esempio, il fatto che la Biblioteca Nazionale Centrale di Roma ha un numero di telefono di riferimento, un numero di fax, un email come pure una PEC può essere descritto nel seguente modo in turtle:


&lt;pre&gt;

contactPoint:Contatti_di_Biblioteca_nazionale_centrale_di_Roma
      a       cis:ContactPoint ;
      rdfs:label &quot;Contatti di: Biblioteca nazionale centrale di Roma&quot;@it ;
      cis:available   openingHoursSpecification:Orari_di_apertura_di_Biblioteca_nazionale_centrale_di_Roma_giovedi ;
      cis:hasCertifiedEmail
              mailto:mbac-bnc-rm@mailcert.beniculturali.it ;
      cis:hasEmail mailto:bnc-rm@beniculturali.it ;
      cis:hasFax &quot;+39064457635  &quot; ;
      cis:hasTelephone &quot;+390649891&quot; .

cissite:Biblioteca_nazionale_centrale
      a       cis:Library , cis:CulturalInstituteOrSite ;
      cis:hasContactPoint contactPoint:Contatti_di_Biblioteca_nazionale_centrale_di_Roma .

&lt;/pre&gt;</dc:description>
        <dc:description xml:lang="en">Individuals of the classes CulturalInstituteOrSite, Event and Site may have a &quot;contact point&quot;, i.e., a phone number, email address, fax, etc. that is used a reference contact.

Additionally, a cantact point might be also declared to be operative with respect to specific hopening hours.

This information is modelled into a knowledge base by using the object property hasContactPoint whose domain can be a CulturalInstituteOrSite, an Event or a Site, and its range is any indifvidual of the class ContactPoint.

For example, the fact that the Biblioteca Nazionale Centrale of Rome has  reference phone and fax number and a email as well as certified email contacts can be described in the following way by using turtle:

&lt;pre&gt;

contactPoint:Contatti_di_Biblioteca_nazionale_centrale_di_Roma
      a       cis:ContactPoint ;
      rdfs:label &quot;Contatti di: Biblioteca nazionale centrale di Roma&quot;@it ;
      cis:available   openingHoursSpecification:Orari_di_apertura_di_Biblioteca_nazionale_centrale_di_Roma_giovedi ;
      cis:hasCertifiedEmail
              mailto:mbac-bnc-rm@mailcert.beniculturali.it ;
      cis:hasEmail mailto:bnc-rm@beniculturali.it ;
      cis:hasFax &quot;+39064457635  &quot; ;
      cis:hasTelephone &quot;+390649891&quot; .

cissite:Biblioteca_nazionale_centrale
      a       cis:Library , cis:CulturalInstituteOrSite ;
      cis:hasContactPoint contactPoint:Contatti_di_Biblioteca_nazionale_centrale_di_Roma .

&lt;/pre&gt;</dc:description>
        <rdfs:comment xml:lang="en">It represents a contact point which consists of phone numbers, e-mail addresses, web sites and their availability where applicable. We recommend the domain experts to specify better during the data production phase which type of contact point is in use (administrative contact point, tourist contact point, etc,).</rdfs:comment>
        <rdfs:comment xml:lang="it">Rappresenta un punto di contatto (racchiude numeri di telefono, fax, indirizzi e-mail, siti web e relative disponibilità ove applicabili). Si raccomanda agli esperti di dominio di aver cura in fase di utilizzo di distinguere ulteriormente il tipo di punto di contatto (turistico, amministrativo, ecc).</rdfs:comment>
        <rdfs:isDefinedBy rdf:resource="http://dati.beniculturali.it/cis/"/>
        <rdfs:label xml:lang="en">Contact Point</rdfs:label>
        <rdfs:label xml:lang="it">Punto di Contatto</rdfs:label>
        <owl:versionInfo xml:lang="it">stabile</owl:versionInfo>
        <owl:versionInfo xml:lang="en">stable</owl:versionInfo>
    </owl:Class>
    


    <!-- http://dati.beniculturali.it/cis/CulturalInstituteOrSite -->


    <owl:Class rdf:about="http://dati.beniculturali.it/cis/CulturalInstituteOrSite">
        <rdfs:subClassOf>
            <owl:Restriction>
                <owl:onProperty rdf:resource="http://dati.beniculturali.it/cis/hasSite"/>
                <owl:someValuesFrom rdf:resource="http://dati.beniculturali.it/cis/Site"/>
            </owl:Restriction>
        </rdfs:subClassOf>
        <rdfs:subClassOf>
            <owl:Restriction>
                <owl:onProperty rdf:resource="http://dati.beniculturali.it/cis/catalogue"/>
                <owl:allValuesFrom rdf:resource="http://dati.beniculturali.it/cis/Catalogue"/>
            </owl:Restriction>
        </rdfs:subClassOf>
        <rdfs:subClassOf>
            <owl:Restriction>
                <owl:onProperty rdf:resource="http://dati.beniculturali.it/cis/hasAccessCondition"/>
                <owl:allValuesFrom rdf:resource="http://dati.beniculturali.it/cis/AccessCondition"/>
            </owl:Restriction>
        </rdfs:subClassOf>
        <rdfs:subClassOf>
            <owl:Restriction>
                <owl:onProperty rdf:resource="http://dati.beniculturali.it/cis/hasContactPoint"/>
                <owl:allValuesFrom rdf:resource="http://dati.beniculturali.it/cis/ContactPoint"/>
            </owl:Restriction>
        </rdfs:subClassOf>
        <rdfs:subClassOf>
            <owl:Restriction>
                <owl:onProperty rdf:resource="http://dati.beniculturali.it/cis/providesService"/>
                <owl:allValuesFrom rdf:resource="http://dati.beniculturali.it/cis/Service"/>
            </owl:Restriction>
        </rdfs:subClassOf>
        <rdfs:subClassOf>
            <owl:Restriction>
                <owl:onProperty rdf:resource="http://dati.beniculturali.it/cis/institutionalName"/>
                <owl:someValuesFrom rdf:resource="http://www.w3.org/2000/01/rdf-schema#Literal"/>
            </owl:Restriction>
        </rdfs:subClassOf>
        <rdfs:subClassOf>
            <owl:Restriction>
                <owl:onProperty rdf:resource="http://dati.beniculturali.it/cis/ISILIdentifier"/>
                <owl:cardinality rdf:datatype="http://www.w3.org/2001/XMLSchema#nonNegativeInteger">1</owl:cardinality>
            </owl:Restriction>
        </rdfs:subClassOf>
        <dc:description rdf:resource="http://dati.beniculturali.it/cis/img/cis.png"/>
        <dc:description xml:lang="en">An example of usage of the class &apos;Cultural Institute or Site&apos; is the following:

&lt;pre&gt;

cissite:Biblioteca_nazionale_centrale
      a       cis:Library , cis:CulturalInstituteOrSite ;
      rdfs:comment &quot;&quot;&quot;La Biblioteca Nazionale Centrale di Roma fu inaugurata il 14 marzo 1876 in un&apos;ala del 
      monumentale Palazzo cinquecentesco del Collegio Romano, sede dell&apos;antica Bibliotheca Secreta o Major dei Gesuiti, 
      che costituì il nucleo originario della nuova istituzione, cui si aggiunsero i fondi manoscritti e a stampa di 69 
      biblioteche conventuali devolute al Regno d&apos;Italia dopo la soppressione delle corporazioni religiose di Roma 
      nel 1873. 
	  Cento anni dopo la Biblioteca venne trasferita nella nuova sede, all&apos;interno della zona archeologica del 
	  Castro Pretorio, fra la Città universitaria e la Stazione Termini, realizzata su progetto degli architetti Massimo
      Castellazzi, Tullio Dell&apos;Anese e Annibale Vitellozzi.&quot;&quot;&quot;@it ;
      rdfs:label &quot;Biblioteca nazionale centrale&quot;@it ;
      cis:ISILIdentifier &quot;IT-RM0267&quot;^^xsd:string ;
      cis:description &quot;&quot;&quot;La Biblioteca Nazionale Centrale di Roma fu inaugurata il 14 marzo 1876 in un&apos;ala del 
      monumentale Palazzo cinquecentesco del Collegio Romano, sede dell&apos;antica Bibliotheca Secreta o Major dei Gesuiti, 
      che costituì il nucleo originario della nuova istituzione, cui si aggiunsero i fondi manoscritti e a stampa di 69 
      biblioteche conventuali devolute al Regno d&apos;Italia dopo la soppressione delle corporazioni religiose di Roma 
      nel 1873. Cento anni dopo la Biblioteca venne trasferita nella nuova sede, all&apos;interno della zona archeologica 
      del Castro Pretorio, fra la Città universitaria e la Stazione Termini, realizzata su progetto degli architetti 
      Massimo Castellazzi, Tullio Dell&apos;Anese e Annibale Vitellozzi.&quot;&quot;&quot;@it ;
      cis:hasAccessCondition
              &lt;http://dati.beniculturali.it/cis/resource/OpeningHoursSpecification/Orari_di_apertura_di_Biblioteca_nazionale_centrale_di_Roma_giovedi&gt; , 
              &lt;http://dati.beniculturali.it/cis/resource/OpeningHoursSpecification/Orari_di_apertura_di_Biblioteca_nazionale_centrale_di_Roma_mercoledi&gt; , 
              &lt;http://dati.beniculturali.it/cis/resource/OpeningHoursSpecification/Orari_di_apertura_di_Biblioteca_nazionale_centrale_di_Roma_lunedi&gt; , 
              &lt;http://dati.beniculturali.it/cis/resource/OpeningHoursSpecification/Orari_di_apertura_di_Biblioteca_nazionale_centrale_di_Roma_martedi&gt; , &lt;http://dati.beniculturali.it/cis/resource/OpeningHoursSpecification/Orari_di_apertura_di_Biblioteca_nazionale_centrale_di_Roma_venerdi&gt; ;
      cis:hasCatalogue &lt;http://dati.beniculturali.it/cis/resource/Catalogue/Catalogo_Generale_%28topografico%29&gt; , &lt;http://dati.beniculturali.it/cis/resource/Catalogue/Catalogo_Generale_%28titoli%29&gt; , &lt;http://dati.beniculturali.it/cis/resource/Catalogue/Catalogo_Generale_%28autore%29&gt; , &lt;http://dati.beniculturali.it/cis/resource/Catalogue/Catalogo_Generale_%28sistematico%29&gt; , &lt;http://dati.beniculturali.it/cis/resource/Catalogue/Catalogo_Generale_%28soggetto%29&gt; ;
      cis:hasCollection collezioni:Patrimonio_di_Biblioteca_nazionale_centrale_di_Roma ;
      cis:hasContactPoint contactPoint:Contatti_di_Biblioteca_nazionale_centrale_di_Roma ;
      cis:hasNameInTime nameInTime:Biblioteca_Nazionale_Centrale ;
      cis:hasSite site:Sede_di_Biblioteca_nazionale_centrale_di_Roma ;
      cis:institutionalName
              &quot;Biblioteca Nazionale Centrale&quot;@it ;
      cis:providesService service:Connessione_WI-FI , service:Visite_guidate , service:ala_per_la_didattica ;
      owl:sameAs   &lt;http://it.dbpedia.org/resource/Biblioteca_Nazionale_Centrale_di_Roma&gt; ;
      cis:institutionalName &quot;&quot;Biblioteca nazionale centrale&quot;@it .

&lt;/pre&gt;</dc:description>
        <dc:description xml:lang="it">Un esempio di utilizzo della classe &quot;Istituto e Luogo della Cultura&quot; è il seguente:

&lt;pre&gt;

cissite:Biblioteca_nazionale_centrale
      a       cis:Library , cis:CulturalInstituteOrSite ;
      rdfs:comment &quot;La Biblioteca Nazionale Centrale di Roma fu inaugurata il 14 marzo 1876 in un&apos;ala del 
      monumentale Palazzo cinquecentesco del Collegio Romano, sede dell&apos;antica Bibliotheca Secreta o Major dei Gesuiti, 
      che costituì il nucleo originario della nuova istituzione, cui si aggiunsero i fondi manoscritti e a stampa di 69 
      biblioteche conventuali devolute al Regno d&apos;Italia dopo la soppressione delle corporazioni religiose di Roma 
      nel 1873. 
	  Cento anni dopo la Biblioteca venne trasferita nella nuova sede, all&apos;interno della zona archeologica del 
	  Castro Pretorio, fra la Città universitaria e la Stazione Termini, realizzata su progetto degli architetti Massimo
      Castellazzi, Tullio Dell&apos;Anese e Annibale Vitellozzi.&quot;&quot;&quot;@it ;
      rdfs:label &quot;Biblioteca nazionale centrale&quot;@it ;
      cis:ISILIdentifier &quot;IT-RM0267&quot;^^xsd:string ;
      cis:description &quot;&quot;La Biblioteca Nazionale Centrale di Roma fu inaugurata il 14 marzo 1876 in un&apos;ala del 
      monumentale Palazzo cinquecentesco del Collegio Romano, sede dell&apos;antica Bibliotheca Secreta o Major dei Gesuiti, 
      che costituì il nucleo originario della nuova istituzione, cui si aggiunsero i fondi manoscritti e a stampa di 69 
      biblioteche conventuali devolute al Regno d&apos;Italia dopo la soppressione delle corporazioni religiose di Roma 
      nel 1873. Cento anni dopo la Biblioteca venne trasferita nella nuova sede, all&apos;interno della zona archeologica 
      del Castro Pretorio, fra la Città universitaria e la Stazione Termini, realizzata su progetto degli architetti 
      Massimo Castellazzi, Tullio Dell&apos;Anese e Annibale Vitellozzi.&quot;&quot;&quot;@it ;
      cis:hasAccessCondition
              &lt;http://dati.beniculturali.it/cis/resource/OpeningHoursSpecification/Orari_di_apertura_di_Biblioteca_nazionale_centrale_di_Roma_giovedi&gt; , 
              &lt;http://dati.beniculturali.it/cis/resource/OpeningHoursSpecification/Orari_di_apertura_di_Biblioteca_nazionale_centrale_di_Roma_mercoledi&gt; , 
              &lt;http://dati.beniculturali.it/cis/resource/OpeningHoursSpecification/Orari_di_apertura_di_Biblioteca_nazionale_centrale_di_Roma_lunedi&gt; , 
              &lt;http://dati.beniculturali.it/cis/resource/OpeningHoursSpecification/Orari_di_apertura_di_Biblioteca_nazionale_centrale_di_Roma_martedi&gt; , &lt;http://dati.beniculturali.it/cis/resource/OpeningHoursSpecification/Orari_di_apertura_di_Biblioteca_nazionale_centrale_di_Roma_venerdi&gt; ;
      cis:hasCatalogue &lt;http://dati.beniculturali.it/cis/resource/Catalogue/Catalogo_Generale_%28topografico%29&gt; , &lt;http://dati.beniculturali.it/cis/resource/Catalogue/Catalogo_Generale_%28titoli%29&gt; , &lt;http://dati.beniculturali.it/cis/resource/Catalogue/Catalogo_Generale_%28autore%29&gt; , &lt;http://dati.beniculturali.it/cis/resource/Catalogue/Catalogo_Generale_%28sistematico%29&gt; , &lt;http://dati.beniculturali.it/cis/resource/Catalogue/Catalogo_Generale_(soggetto)&gt; ;
      cis:hasCollection collezioni:Patrimonio_di_Biblioteca_nazionale_centrale_di_Roma ;
      cis:hasContactPoint contactPoint:Contatti_di_Biblioteca_nazionale_centrale_di_Roma ;
      cis:hasNameInTime nameInTime:Biblioteca_Nazionale_Centrale ;
      cis:hasSite site:Sede_di_Biblioteca_nazionale_centrale_di_Roma ;
      cis:institutionalName
              &quot;Biblioteca Nazionale Centrale&quot;@it ;
      cis:providesService service:Connessione_WI-FI , service:Visite_guidate , service:ala_per_la_didattica ;
      owl:sameAs &lt;http://it.dbpedia.org/resource/Biblioteca_Nazionale_Centrale_di_Roma&gt; ;
       cis:institutionalName &quot;Biblioteca nazionale centrale&quot;@it .

&lt;/pre&gt;</dc:description>
        <rdfs:comment xml:lang="it">Sono istituti e luoghi della cultura i musei, le biblioteche e gli archivi, le aree e i parchi archeologici, i complessi monumentali. Gli istituti e luoghi e della cultura che appartengono a soggetti pubblici sono destinati alla pubblica fruizione ed espletano un servizio pubblico. Le strutture espositive e di consultazione nonché i luoghi della cultura che appartengono a soggetti privati e sono aperti al pubblico espletano un servizio privato di utilità sociale.</rdfs:comment>
        <rdfs:comment xml:lang="en">The class Cultural Institute or Site represents museums, libraries, archive holders, archaeologic areas and parks, monumental areas. The cultural institutes of sites that are owned by public bodies are meant to offer public services. The cultural institutes or sites that are owned by private subjects, and are open to the public, offer a public and societal service.</rdfs:comment>
        <rdfs:isDefinedBy rdf:resource="http://dati.beniculturali.it/cis/"/>
        <rdfs:label xml:lang="en">Cultural Institute or Site</rdfs:label>
        <rdfs:label xml:lang="it">Istituto e Luogo Della Cultura</rdfs:label>
        <owl:versionInfo xml:lang="it">stabile</owl:versionInfo>
        <owl:versionInfo xml:lang="en">stable</owl:versionInfo>
    </owl:Class>
    


    <!-- http://dati.beniculturali.it/cis/DayOfWeek -->


    <owl:Class rdf:about="http://dati.beniculturali.it/cis/DayOfWeek">
        <dc:description rdf:resource="http://dati.beniculturali.it/cis/img/openingHoursSpecification.png"/>
        <dc:description xml:lang="en">An example of usage of the class cis:DayOfTheWeek is the following:

&lt;pre&gt;

orari:Orari_di_apertura_di_Biblioteca_nazionale_centrale_di_Roma_giovedi
      a       cis:OpeningHoursSpecification ;
      rdfs:label &quot;Opening Hours of Biblioteca nazionale centrale di Roma - thursday&quot;@en , 
      &quot;Orari di apertura di Biblioteca nazionale centrale di Roma - giovedì&quot;@it ;
      cis:closes &quot;19:00:00&quot;^^xsd:time ;
      cis:hasAdmissionType addmissionType:Tipo_di_apertura_al_pubblico ;
      cis:hasDayOfWeek cis:Thursday ;
      cis:opens &quot;08:30:00&quot;^^xsd:time .

&lt;/pre&gt;

For the complete example see the class cis:OpeningHoursSpecification</dc:description>
        <dc:description xml:lang="it">Un esempio di utilizzo della classe cis:DayOfTheWeek è il seguente:

&lt;pre&gt;

orari:Orari_di_apertura_di_Biblioteca_nazionale_centrale_di_Roma_giovedi
      a       cis:OpeningHoursSpecification ;
      rdfs:label &quot;Opening Hours of Biblioteca nazionale centrale di Roma - thursday&quot;@en , 
      &quot;Orari di apertura di Biblioteca nazionale centrale di Roma - giovedì&quot;@it ;
      cis:closes &quot;19:00:00&quot;^^xsd:time ;
      cis:hasAdmissionType addmissionType:Tipo_di_apertura_al_pubblico ;
      cis:hasDayOfWeek cis:Thursday ;
      cis:opens &quot;08:30:00&quot;^^xsd:time .

&lt;/pre&gt;

Per un esempio più completo si veda la classe cis:OpeningHoursSpecification</dc:description>
        <rdfs:comment xml:lang="it">Classe che rappresenta l&apos;insieme dei giorni della settimana.</rdfs:comment>
        <rdfs:comment xml:lang="en">This class represents the set of all the days of the week.</rdfs:comment>
        <rdfs:isDefinedBy rdf:resource="http://dati.beniculturali.it/cis/"/>
        <rdfs:label xml:lang="en">Day of the Week</rdfs:label>
        <rdfs:label xml:lang="it">Giorno della settimana </rdfs:label>
        <owl:versionInfo xml:lang="en">unstable</owl:versionInfo>
        <owl:versionInfo xml:lang="it">versione non definitiva</owl:versionInfo>
    </owl:Class>
    


    <!-- http://dati.beniculturali.it/cis/GeographicalFeature -->


    <owl:Class rdf:about="http://dati.beniculturali.it/cis/GeographicalFeature">
        <rdfs:subClassOf>
            <owl:Restriction>
                <owl:onProperty rdf:resource="http://dati.beniculturali.it/cis/toponym"/>
                <owl:someValuesFrom rdf:resource="http://www.w3.org/2000/01/rdf-schema#Literal"/>
            </owl:Restriction>
        </rdfs:subClassOf>
        <dc:description rdf:resource="http://dati.beniculturali.it/cis/img/geographicalArea.png"/>
        <dc:description xml:lang="it">Questa classe consente di descrivere un&apos;area geografica. 

Le aree geografiche sono semrep associate a individui della classe Sede attraverso la proprietà ha locazione geografica (dominio Sede e codonimio Area Geografica).

Un area geografica è descritta dall&apos;insieme di individui della classe geometria. Un individuo della classe geometria è descritto utilizzando le coordinate del sistema di riferimento come per esempio WGS84. E? univocamente identificata da latitudine e longitudine. Questo significa che un area geografica può essere un punto, una linea o un poligono. 

Per esempio, il seguente frammento di codice in turtle fornisce rappresenta un area geografica corrispondente alla sede della Biblioteca Centrale di Roma.

&lt;pre&gt;


site:Sede_di_Biblioteca_nazionale_centrale_di_Roma
      a       cis:Site ;
      cis:hasGeographicalLocation
              geographicalArea:Comune_di_Roma ;
      cis:isSiteOf cissite:Biblioteca_nazionale_centrale ;
      cis:name &quot;Biblioteca nazionale centrale di Roma&quot;@it .

geographicalArea:Comune_di_Roma
      a       cis:GeographicalArea ;
      rdfs:label &quot;Comune di Roma&quot;@it ;
      cis:toponym &quot;Roma&quot; ;
      owl:sameAs      &lt;http://spcdata.digitpa.gov.it/Comune/H501&gt; , &lt;http://datiopen.istat.it/odi/risorsa/territorio/comuni/Roma_58091&gt; ;
      hasGeometry geometry:Comune_di_Roma .

geometry:Comune_di_Roma
      a       cis:Geometry ;
      geo:lat &quot;41.906784&quot; ;
      geo:long &quot;12.504962&quot; .
	
&lt;/pre&gt;</dc:description>
        <dc:description xml:lang="en">This class allows describing a geographical area.
Geographical areas are always associated with individuals of the class &apos;Site&apos; by means of the object property hasGeographicalLocation (domain Site and range &apos;Geographical Area&apos;).

A geographical area is described by a set of individuals of the class Geometry. A individual of the class Geometry is described by using a coordinate system related to Earth such as WGS84. It is univocally identified by lat/long. This means that a geographical area can be a point, a line or a polygon.

For example, the following snippet provides a turtle model that represents a Geographical Area corresponding to the Site of the Biblioteca Centrale di Roma.

&lt;pre&gt;


site:Sede_di_Biblioteca_nazionale_centrale_di_Roma
      a       cis:Site ;
      cis:hasGeographicalLocation
              geographicalArea:Comune_di_Roma ;
      cis:isSiteOf cissite:Biblioteca_nazionale_centrale ;
      cis:name &quot;Biblioteca nazionale centrale di Roma&quot;@it .

geographicalArea:Comune_di_Roma
      a       cis:GeographicalArea ;
      rdfs:label &quot;Comune di Roma&quot;@it ;
      cis:toponym &quot;Roma&quot; ;
      owl:sameAs      &lt;http://spcdata.digitpa.gov.it/Comune/H501&gt; , &lt;http://datiopen.istat.it/odi/risorsa/territorio/comuni/Roma_58091&gt; ;
      hasGeometry geometry:Comune_di_Roma .

geometry:Comune_di_Roma
      a       cis:Geometry ;
      geo:lat &quot;41.906784&quot; ;
      geo:long &quot;12.504962&quot; .
	
&lt;/pre&gt;</dc:description>
        <rdfs:comment xml:lang="en">It represents a geographical feature. It can be used to model a municipality or an area across different administrative areas.</rdfs:comment>
        <rdfs:comment xml:lang="it">Rappresenta una caratteristica  geografica. Può essere usata per rappresentare un comune, o un&apos;area che ricomprendere diverse aree ammistrative.</rdfs:comment>
        <rdfs:isDefinedBy rdf:resource="http://dati.beniculturali.it/cis/"/>
        <rdfs:label xml:lang="it">Area Geografica</rdfs:label>
        <rdfs:label xml:lang="en">Geographical Area</rdfs:label>
        <owl:versionInfo xml:lang="it">stabile</owl:versionInfo>
        <owl:versionInfo xml:lang="en">stable</owl:versionInfo>
    </owl:Class>
    


    <!-- http://dati.beniculturali.it/cis/Geometry -->


    <owl:Class rdf:about="http://dati.beniculturali.it/cis/Geometry">
        <rdfs:subClassOf>
            <owl:Restriction>
                <owl:onProperty rdf:resource="http://dati.beniculturali.it/cis/hasLat"/>
                <owl:allValuesFrom rdf:resource="http://www.w3.org/2001/XMLSchema#decimal"/>
            </owl:Restriction>
        </rdfs:subClassOf>
        <rdfs:subClassOf>
            <owl:Restriction>
                <owl:onProperty rdf:resource="http://dati.beniculturali.it/cis/hasLong"/>
                <owl:allValuesFrom rdf:resource="http://www.w3.org/2001/XMLSchema#decimal"/>
            </owl:Restriction>
        </rdfs:subClassOf>
        <dc:description xml:lang="en">An example of usage of the class cis:Geometry is the following:
&lt;pre&gt;

geometry:Museo_di_Capodimonte_Geometry
      a       cis:Geometry ;
      rdfs:label &quot;Coordinate geografiche della sede di Museo di Capodimonte&quot;@it;
      cis:hasLat &quot;40.867424&quot; ;
      cis:geometryType &quot;Point&quot;;
      cis:geoMethodology &quot;Satellite data georeferentiation&quot; ;
      cis:hasLong &quot;14.249192&quot;.

&lt;/pre&gt;

For a complete example refer to the class cis:GeographicalFeature</dc:description>
        <dc:description xml:lang="it">Un esempio di utilizzo della classe cis:Geomery è il seguente:
&lt;pre&gt;

geometry:Museo_di_Capodimonte_Geometry
      a       cis:Geometry ;
      rdfs:label &quot;Coordinate geografiche della sede di Museo di Capodimonte&quot;@it;
      cis:hasLat &quot;40.867424&quot; ;
      cis:geometryType &quot;Point&quot;;
      cis:geoMethodology &quot;Satellite data georeferentiation&quot; ;
      cis:hasLong &quot;14.249192&quot;.

&lt;/pre&gt;

Per un esempio complete si veda la classe cis:GeographicalFeature</dc:description>
        <rdfs:comment xml:lang="en">It represents a geometry which is typically described by using a coordinate system related to Earth such as WGS84. It is univocally identified by lat/long</rdfs:comment>
        <rdfs:comment xml:lang="it">Rappresenta una geometria tipicamente descritto utilizzando un sistema di coordinate geografiche come per esempio WGS84. Univocamente identificato da Lat/Long</rdfs:comment>
        <rdfs:isDefinedBy rdf:resource="http://dati.beniculturali.it/cis/"/>
        <rdfs:label xml:lang="it">Geometria</rdfs:label>
        <rdfs:label xml:lang="en">Geometry</rdfs:label>
        <owl:versionInfo xml:lang="it">stabile</owl:versionInfo>
        <owl:versionInfo xml:lang="en">stable</owl:versionInfo>
    </owl:Class>
    


    <!-- http://dati.beniculturali.it/cis/GovernamentalAdministrativeArea -->


    <owl:Class rdf:about="http://dati.beniculturali.it/cis/GovernamentalAdministrativeArea">
        <rdfs:subClassOf rdf:resource="http://dati.beniculturali.it/cis/GeographicalFeature"/>
        <dc:description xml:lang="en">An example of usage of the class cis:GovernamentalAdministrativeArea is the following:

&lt;pre&gt;

gaa:Lazio
    a cis:GovernamentalAdministrativeArea ;
    rdfs:label &quot;Lazio&quot; ;
    cis:toponym &quot;Lazio&quot; ;
    cis:hasISTATCode &quot;12&quot; .

&lt;/pre&gt;</dc:description>
        <dc:description xml:lang="it">Un esempio di utilizzo della classe cis:GovernamentalAdministrativeArea è il seguente:
&lt;pre&gt;

gaa:Lazio
    a cis:GovernamentalAdministrativeArea ;
    rdfs:&quot;Lazio&quot;;;
    cis:toponym &quot;Lazio&quot;;;
    cis:hasISTATCode &quot;12&quot; .

&lt;/pre&gt;</dc:description>
        <rdfs:comment xml:lang="it">Questa classe rappresenta un&apos;area amministrativa territoriale statale gestita tipicamente da un organismo pubblico. Essa può essere una Regione, una Provincia, un Comune, un area sub comunale, etc.</rdfs:comment>
        <rdfs:comment xml:lang="en">This class represents an administrative geographical area that is typically managed by a public body. It can be a Region, a Municipality, a Province, a sub-municipality area, etc.</rdfs:comment>
        <rdfs:isDefinedBy rdf:resource="http://dati.beniculturali.it/cis/"/>
        <rdfs:label xml:lang="it">Area Amministrativa statale</rdfs:label>
        <rdfs:label xml:lang="en">Governamental Administrative Area</rdfs:label>
        <owl:versionInfo xml:lang="it">stabile</owl:versionInfo>
        <owl:versionInfo xml:lang="en">stable</owl:versionInfo>
    </owl:Class>
    


    <!-- http://dati.beniculturali.it/cis/Library -->


    <owl:Class rdf:about="http://dati.beniculturali.it/cis/Library">
        <rdfs:subClassOf rdf:resource="http://dati.beniculturali.it/cis/CulturalInstituteOrSite"/>
        <rdfs:isDefinedBy>http://dati.beniculturali.it/cis/</rdfs:isDefinedBy>
        <rdfs:label xml:lang="en">Library</rdfs:label>
    </owl:Class>
    


    <!-- http://dati.beniculturali.it/cis/OpeningHoursSpecification -->


    <owl:Class rdf:about="http://dati.beniculturali.it/cis/OpeningHoursSpecification">
        <rdfs:subClassOf rdf:resource="http://dati.beniculturali.it/cis/AccessCondition"/>
        <rdfs:subClassOf>
            <owl:Restriction>
                <owl:onProperty rdf:resource="http://dati.beniculturali.it/cis/hasDayOfWeek"/>
                <owl:allValuesFrom rdf:resource="http://dati.beniculturali.it/cis/DayOfWeek"/>
            </owl:Restriction>
        </rdfs:subClassOf>
        <rdfs:subClassOf>
            <owl:Restriction>
                <owl:onProperty rdf:resource="http://dati.beniculturali.it/cis/closes"/>
                <owl:allValuesFrom rdf:resource="http://www.w3.org/2001/XMLSchema#time"/>
            </owl:Restriction>
        </rdfs:subClassOf>
        <rdfs:subClassOf>
            <owl:Restriction>
                <owl:onProperty rdf:resource="http://dati.beniculturali.it/cis/opens"/>
                <owl:allValuesFrom rdf:resource="http://www.w3.org/2001/XMLSchema#time"/>
            </owl:Restriction>
        </rdfs:subClassOf>
        <dc:description rdf:resource="http://dati.beniculturali.it/cis/img/openingHoursSpecification.png"/>
        <dc:description xml:lang="en">Individuals of this class specify a particula access conditions, i.e., the opening hours of a &apos;Cultural Institute or Site&apos; or an &apos;Event&apos;.

Opening hours are represented in terms of:
   * opening time (cf. property opens);
   * closing time (cf. property closes);
   * the day of the week that the opening specification refers to (cf. property hasDayOfWeek);
   * the admission type, e.g. weekly, monthly, daily, etc (cf. property hasAdmmissionType).

An example in turtle is the following:

&lt;pre&gt;

cissite:Biblioteca_nazionale_centrale
      a       cis:Library , cis:CulturalInstituteOrSite ;
      cis:hasAccessCondition            orari:Orari_di_apertura_di_Biblioteca_nazionale_centrale_di_Roma_giovedi

orari:Orari_di_apertura_di_Biblioteca_nazionale_centrale_di_Roma_giovedi
      a       cis:OpeningHoursSpecification ;
      rdfs:label &quot;Opening Hours of Biblioteca nazionale centrale di Roma - thursday&quot;@en , 
      &quot;Orari di apertura di Biblioteca nazionale centrale di Roma - giovedì&quot;@it ;
      cis:closes &quot;19:00:00&quot;^^xsd:time ;
      cis:hasAdmissionType          addmissionType:Tipo_di_apertura_al_pubblico ;
      cis:hasDayOfWeek cis:Thursday ;
      cis:opens &quot;08:30:00&quot;^^xsd:time .

admissionType:Tipo_di_apertura_al_pubblico
      a       cis:AdmissionType ;
      cis:description &quot;daily&quot; .

&lt;/pre&gt;</dc:description>
        <dc:description xml:lang="it">Individui di questa classe specificano particolari condizioni di accesso ai luoghi della cultura o eventi, i.e., gli orari di apertura dei luoghi o degli eventi.

Gli orari di apertura sono espressi in termini di 
 * orario apertura (con la proprietà &quot;apre&quot;)
 * orario di chiusura (con la proprietà &quot;chiude&quot;)
 * il giorno della settimana a cui l&apos;orario di apertura si riferisce (con la proprietà ha giorno della settimana)
 * il tipo di apertura (settimanale, mensile, giornaliera, ecc) (con la proprietà ha tipo di apertura)

Un esempio in turle è il seguente:
&lt;pre&gt;

cissite:Biblioteca_nazionale_centrale
      a       cis:Library , cis:CulturalInstituteOrSite ;
      cis:hasAccessCondition            orari:Orari_di_apertura_di_Biblioteca_nazionale_centrale_di_Roma_giovedi

orari:Orari_di_apertura_di_Biblioteca_nazionale_centrale_di_Roma_giovedi
      a       cis:OpeningHoursSpecification ;
      rdfs:label &quot;Opening Hours of Biblioteca nazionale centrale di Roma - thursday&quot;@en , 
      &quot;Orari di apertura di Biblioteca nazionale centrale di Roma - giovedì&quot;@it ;
      cis:closes &quot;19:00:00&quot;^^xsd:time ;
      cis:hasAdmissionType          addmissionType:Tipo_di_apertura_al_pubblico ;
      cis:hasDayOfWeek cis:Thursday ;
      cis:opens &quot;08:30:00&quot;^^xsd:time .

admissionType:Tipo_di_apertura_al_pubblico
      a       cis:AdmissionType ;
      cis:description &quot;daily&quot; .

&lt;/pre&gt;</dc:description>
        <rdfs:comment xml:lang="en">It represents the opening hours specification </rdfs:comment>
        <rdfs:comment xml:lang="it">Rappresenta gli orari di apertura</rdfs:comment>
        <rdfs:label xml:lang="en">Opening Hours Specification</rdfs:label>
        <rdfs:label xml:lang="it">Orari di Apertura</rdfs:label>
        <owl:versionInfo xml:lang="it">stabile</owl:versionInfo>
        <owl:versionInfo xml:lang="en">stable</owl:versionInfo>
    </owl:Class>
    


    <!-- http://dati.beniculturali.it/cis/Service -->


    <owl:Class rdf:about="http://dati.beniculturali.it/cis/Service">
        <rdfs:subClassOf>
            <owl:Restriction>
                <owl:onProperty rdf:resource="http://dati.beniculturali.it/cis/hasContactPoint"/>
                <owl:allValuesFrom rdf:resource="http://dati.beniculturali.it/cis/ContactPoint"/>
            </owl:Restriction>
        </rdfs:subClassOf>
        <rdfs:subClassOf>
            <owl:Restriction>
                <owl:onProperty rdf:resource="http://dati.beniculturali.it/cis/isProvidedBy"/>
                <owl:allValuesFrom rdf:resource="http://dati.beniculturali.it/cis/CulturalInstituteOrSite"/>
            </owl:Restriction>
        </rdfs:subClassOf>
        <rdfs:subClassOf>
            <owl:Restriction>
                <owl:onProperty rdf:resource="http://dati.beniculturali.it/cis/name"/>
                <owl:someValuesFrom rdf:resource="http://www.w3.org/2000/01/rdf-schema#Literal"/>
            </owl:Restriction>
        </rdfs:subClassOf>
        <dc:description xml:lang="en">A Cultural Institute or Site (CIS) might offer a variety of services (e.g., Wi-Fi Handicapped access, cafeteria, etc.).

These services are represented as individuals of the class &apos;Service&apos; and they are in relationship with a CIS by means of the object property providesService.

The following is an example expressed by using the turtle syntax:

&lt;pre&gt;

service:Caffetteria
      a       cis:Service ;
      cis:name &quot;Caffetteria&quot; .


service:Connessione_WI-FI
      a       cis:Service ;
      cis:name &quot;Connessione WI-FI&quot; .


cissite:Biblioteca_nazionale_centrale
      a       cis:Library , cis:CulturalInstituteOrSite ;
      cis:providesService service:Caffetteria, service:Connessione_WI-FI.

&lt;/pre&gt;</dc:description>
        <dc:description xml:lang="it">Un istituto della cultura può offrire una serie di servizi (e.g., Wi-Fi, accesso ai disabili, caffetteria, ecc.).

Questi servizi sono rappresentati da individui della classe &quot;Servizio&quot; e sono in relazione con l&apos;istituto della cultural attraverso la proprietà &quot;fornisce servizio&quot;.

Il seguente esempio mostra in turtle l&apos;uso della classe servizio:

&lt;pre&gt;

service:Caffetteria
      a       cis:Service ;
      cis:name &quot;Caffetteria&quot; .


service:Connessione_WI-FI
      a       cis:Service ;
      cis:name &quot;Connessione WI-FI&quot; .


cissite:Biblioteca_nazionale_centrale
      a       cis:Library , cis:CulturalInstituteOrSite ;
      cis:providesService service:Caffetteria, service:Connessione_WI-FI.

&lt;/pre&gt;</dc:description>
        <rdfs:comment xml:lang="en">It represents a service that is provided by the Cultural Institute or Site. For instance, a service can be: the presence of a restaurant internal to the Cultural Institute or Site, the uso of an educational room, the use of a free wifi connection</rdfs:comment>
        <rdfs:comment xml:lang="it">Rappresenta un servizio offerto da un istituto e luogo della cultura. Per esempio, un servizio può essere: la presenza di un ristorante interno al luogo, l&apos;uso una sala didattica, l&apos;uso di una connessione wifi libera, ecc.</rdfs:comment>
        <rdfs:isDefinedBy rdf:resource="http://dati.beniculturali.it/cis/"/>
        <rdfs:label xml:lang="en">Service</rdfs:label>
        <rdfs:label xml:lang="it">Servizio</rdfs:label>
        <owl:versionInfo xml:lang="it">stabile</owl:versionInfo>
        <owl:versionInfo xml:lang="en">stable</owl:versionInfo>
    </owl:Class>
    


    <!-- http://dati.beniculturali.it/cis/Site -->


    <owl:Class rdf:about="http://dati.beniculturali.it/cis/Site">
        <rdfs:subClassOf>
            <owl:Restriction>
                <owl:onProperty rdf:resource="http://dati.beniculturali.it/cis/hasAddress"/>
                <owl:someValuesFrom rdf:resource="http://dati.beniculturali.it/cis/Address"/>
            </owl:Restriction>
        </rdfs:subClassOf>
        <rdfs:subClassOf>
            <owl:Restriction>
                <owl:onProperty rdf:resource="http://dati.beniculturali.it/cis/hasGeographicalLocation"/>
                <owl:someValuesFrom rdf:resource="http://dati.beniculturali.it/cis/GeographicalFeature"/>
            </owl:Restriction>
        </rdfs:subClassOf>
        <rdfs:subClassOf>
            <owl:Restriction>
                <owl:onProperty rdf:resource="http://dati.beniculturali.it/cis/isSiteOf"/>
                <owl:someValuesFrom rdf:resource="http://dati.beniculturali.it/cis/CulturalInstituteOrSite"/>
            </owl:Restriction>
        </rdfs:subClassOf>
        <rdfs:subClassOf>
            <owl:Restriction>
                <owl:onProperty rdf:resource="http://dati.beniculturali.it/cis/hasContactPoint"/>
                <owl:allValuesFrom rdf:resource="http://dati.beniculturali.it/cis/ContactPoint"/>
            </owl:Restriction>
        </rdfs:subClassOf>
        <rdfs:subClassOf>
            <owl:Restriction>
                <owl:onProperty rdf:resource="http://dati.beniculturali.it/cis/hasGeometry"/>
                <owl:allValuesFrom rdf:resource="http://dati.beniculturali.it/cis/Geometry"/>
            </owl:Restriction>
        </rdfs:subClassOf>
        <rdfs:subClassOf>
            <owl:Restriction>
                <owl:onProperty rdf:resource="http://dati.beniculturali.it/cis/name"/>
                <owl:someValuesFrom rdf:resource="http://www.w3.org/2000/01/rdf-schema#Literal"/>
            </owl:Restriction>
        </rdfs:subClassOf>
        <dc:description xml:lang="en">A site is always associated with an individual of the class &apos;Cultural Institute or Site&apos; (CIS) by means of the object property hasSite.

A site is characterised by the following properties:

 * hasAddress that allows associating the site with an indidivdual of the class Address, this latter providing the description of the address;
 * hasContactPoint that associates the site with an individual identifying a contact point;
 * hasGeographicalLocation for relating the site to the description of its geographical features, that, in turn, is represented by means of an individual of the class &apos;Geographical Area&apos;;
 * name that is the datatype property for associating the site with a literal expressing a name;
 * isSiteOf that is the inverse property of hasSite.

The following is an example of a Site and its association with a CIS

&lt;pre&gt;


site:Sede_di_Biblioteca_nazionale_centrale_di_Roma
      a       cis:Site ;
      rdfs:label &quot;Sede Biblioteca nazionale centrale di Roma&quot;@it ;
      cis:hasAddress address:Indirizzo_della_sede_di_Biblioteca_nazionale_centrale_di_Roma ;
      cis:hasContactPoint contactPoint:Contatti_di_Biblioteca_nazionale_centrale_di_Roma ;
      cis:hasGeographicalLocation
              geographicalFeature:Comune_di_Roma ;
      cis:isSiteOf cissite:Biblioteca_nazionale_centrale ;
      cis:name &quot;Sede di: Biblioteca nazionale centrale di Roma&quot;@it .

cissite:Biblioteca_nazionale_centrale
      a       cis:Library , cis:CulturalInstituteOrSite ;
      cis:hasSite site:Sede_di_Biblioteca_nazionale_centrale_di_Roma .

&lt;/pre&gt;</dc:description>
        <dc:description xml:lang="it">Una sede è sempre associata agli individui della classe &quot;Istituto e Luogo della Cultura&quot; attraverso la proprietà ha sede.

Una sede è caratterizzata dalle seguenti proprietà:
 * ha indirizzo: consente di associare una sede con un individuo della classe indirizzo che fornisce la descrizione dell&apos;indirizzo;
 * ha punto di contatto: consente di associare una sede con un individuo che identifica un punto di contatto;
 * ha locazione geografica: consente di associare la sede con la descrizione dell&apos;area geografica 
* nome: una proprietà che consente di specificare il nome della sede
* è sede di: la proprietà inversa di ha sede

Il seguente esempio in turle mostra una sede associata a un istituto e luogo della cultura:

&lt;pre&gt;


site:Sede_di_Biblioteca_nazionale_centrale_di_Roma
      a       cis:Site ;
      rdfs:label &quot;Sede Biblioteca nazionale centrale di Roma&quot;@it ;
      cis:hasAddress address:Indirizzo_della_sede_di_Biblioteca_nazionale_centrale_di_Roma ;
      cis:hasContactPoint contactPoint:Contatti_di_Biblioteca_nazionale_centrale_di_Roma ;
      cis:hasGeographicalLocation
              geographicalFeature:Comune_di_Roma ;
      cis:isSiteOf cissite:Biblioteca_nazionale_centrale ;
      cis:name &quot;Sede di: Biblioteca nazionale centrale di Roma&quot;@it .

cissite:Biblioteca_nazionale_centrale
      a       cis:Library , cis:CulturalInstituteOrSite ;
      cis:hasSite site:Sede_di_Biblioteca_nazionale_centrale_di_Roma .

&lt;/pre&gt;</dc:description>
        <rdfs:comment xml:lang="en">It represents a georeferenced physical site related to the Cultural Institute or Site. A Cultural Institute or Site can be located in more than one physical site. For instance, a Site can be &quot;Palazzo Venezia&quot; which is the site of the &quot;Museum of Palazzo Venezia&quot; and of &quot;Library of Archaelogy and Art History&quot;.</rdfs:comment>
        <rdfs:comment xml:lang="it">Rappresenta un luogo fisico georeferenziato relativo all&apos;Istituto e luogo della Cultura. Un Istituto e Luogo della Cultura può avere più di un luogo fisico associato. Nell&apos;ambito dell&apos;Istituto Centrale per il Catalogo e la Documentazione (ICC)D) tale concetto rappresenta il contenitore fisico. Per esempio, un luogo fisico può essere &quot;Palazzo Venezia&quot; dove ha sede il &quot;Museo Nazionale di Palazzo Venezia&quot; o la &quot;Biblioteca di Archeologia e Storia dell&apos;Arte&quot;.</rdfs:comment>
        <rdfs:isDefinedBy rdf:resource="http://dati.beniculturali.it/cis/"/>
        <rdfs:label xml:lang="it">Sede</rdfs:label>
        <rdfs:label xml:lang="en">Site</rdfs:label>
        <owl:versionInfo xml:lang="it">stabile</owl:versionInfo>
        <owl:versionInfo xml:lang="en">stable</owl:versionInfo>
    </owl:Class>
    


    <!-- http://dati.beniculturali.it/cis/TemporaryClosure -->


    <owl:Class rdf:about="http://dati.beniculturali.it/cis/TemporaryClosure">
        <rdfs:subClassOf rdf:resource="http://dati.beniculturali.it/cis/AccessCondition"/>
        <rdfs:subClassOf>
            <owl:Restriction>
                <owl:onProperty rdf:resource="http://dati.beniculturali.it/cis/hasReason"/>
                <owl:allValuesFrom rdf:resource="http://www.w3.org/2000/01/rdf-schema#Literal"/>
            </owl:Restriction>
        </rdfs:subClassOf>
        <dc:description xml:lang="en">A temporary closure is a subclass of &apos;AccessCondition&apos; whose individuals provide information about a temporary closure.
These individuals are described in terms of:
 * the closure date (cf. property hasDate);
 * the reason about the temporary closure (cf. property hasReason);
 * the type associated with the temporary closure (cf. property hasTemporaryClosureType).

An example in turtle is the following:

&lt;pre&gt;
cissite:Biblioteca_nazionale_centrale
      a       cis:Library , cis:CulturalInstituteOrSite ;
      cis:hasAccessCondition            orari:Chiusura_estiva_di_Biblioteca_nazionale_centrale_di_Roma

orari:Chiusura_estiva_di_Biblioteca_nazionale_centrale_di_Roma
      cis:hasDate &quot;2015-08-15&quot;^^xsd:dateTime ;
      cis:hasReason &quot;Chiusura estiva&quot; ;
&lt;/pre&gt;</dc:description>
        <dc:description xml:lang="it">La chiusura temporanea è una sottoclasse di Condizioni di accesso i cui individui forniscono informazioni sulla chiusura temporanea.

Gli individui sono descritti in termini di:
 * data di chiusura (con la proprietà ha data);
 * la motivazione per la chiusura (con la proprietà ha motivazione)
 * il tipo associato con la chiusura temporanea (con la proprietà ha tipo chiusura temporanea)

Un esempio è il seguente:
&lt;pre&gt;
cissite:Biblioteca_nazionale_centrale
      a       cis:Library , cis:CulturalInstituteOrSite ;
      cis:hasAccessCondition            orari:Chiusura_estiva_di_Biblioteca_nazionale_centrale_di_Roma

orari:Chiusura_estiva_di_Biblioteca_nazionale_centrale_di_Roma
      cis:hasDate &quot;2015-08-15&quot;^^xsd:dateTime ;
      cis:hasReason &quot;Chiusura estiva&quot; ;
&lt;/pre&gt;</dc:description>
        <rdfs:comment xml:lang="en">It represents the information on the temporary closure </rdfs:comment>
        <rdfs:comment xml:lang="it">Rappresenta le informazioni sulla chiusura temporanea</rdfs:comment>
        <rdfs:label xml:lang="it">Chiusura Temporanea</rdfs:label>
        <rdfs:label xml:lang="en">Temporary Closure</rdfs:label>
        <owl:versionInfo xml:lang="it">stabile</owl:versionInfo>
        <owl:versionInfo>stable</owl:versionInfo>
    </owl:Class>
    


    <!-- http://dati.beniculturali.it/cis/TimeInterval -->


    <owl:Class rdf:about="http://dati.beniculturali.it/cis/TimeInterval">
        <rdfs:subClassOf>
            <owl:Restriction>
                <owl:onProperty rdf:resource="http://dati.beniculturali.it/cis/endDate"/>
                <owl:someValuesFrom rdf:resource="http://www.w3.org/2001/XMLSchema#dateTime"/>
            </owl:Restriction>
        </rdfs:subClassOf>
        <rdfs:subClassOf>
            <owl:Restriction>
                <owl:onProperty rdf:resource="http://dati.beniculturali.it/cis/startDate"/>
                <owl:allValuesFrom rdf:resource="http://www.w3.org/2001/XMLSchema#dateTime"/>
            </owl:Restriction>
        </rdfs:subClassOf>
        <dc:description xml:lang="en">An example of usage of the class cis:TimeInterval is the following:

&lt;pre&gt;

timeInteval:Andrea_De_Pasquale_DirectorOfBibliotecaNazionaleCentrale_20130101_20161231
    a cis:TimeInterval ;
    rdfs:label &quot;Andrea De Pasquale director of Biblioteca Nazionale from 2013-01-01 to 2016-12-31&quot;@en ;
    cis:startDate &quot;2013-01-01&quot;^^xsd:dateTime ;
    cis:endDate &quot;2016-12-31&quot;^^xsd:dateTime .

&lt;/pre&gt;</dc:description>
        <dc:description xml:lang="it">Un esempio di utilizzo della classe cis:TimeInterval è il seguente:

&lt;pre&gt;

timeInteval:Andrea_De_Pasquale_DirectorOfBibliotecaNazionaleCentrale_20130101_20161231
    a cis:TimeInterval ;
    rdfs:label &quot;Andrea De Pasquale director of Biblioteca Nazionale from 2013-01-01 to 2016-12-31&quot;@en ;
    cis:startDate &quot;2013-01-01&quot;^^xsd:dateTime ;
    cis:endDate &quot;2016-12-31&quot;^^xsd:dateTime .

&lt;/pre&gt;</dc:description>
        <rdfs:comment xml:lang="en">It represents a temporal interval</rdfs:comment>
        <rdfs:comment xml:lang="it">Rappresenta un intervallo temporale.</rdfs:comment>
        <rdfs:isDefinedBy rdf:resource="http://dati.beniculturali.it/cis/"/>
        <rdfs:label xml:lang="it">Intervallo di Tempo</rdfs:label>
        <rdfs:label xml:lang="en">Time Interval</rdfs:label>
        <owl:versionInfo xml:lang="it">stabile</owl:versionInfo>
        <owl:versionInfo xml:lang="en">stable</owl:versionInfo>
    </owl:Class>
    


    <!-- http://datos.bne.es/def/C1001 -->


    <owl:Class rdf:about="http://datos.bne.es/def/C1001">
        <rdfs:comment xml:lang="en">A work is an abstract entity; there is no single material object one can point to as the work. We recognize the work through individual realizations or expressions of the work, but the work itself exists only in the commonality of content between and among the various expressions of the work. Because the notion of a work is abstract, it is difficult to define precise boundaries for the entity. The concept of what constitutes a work and where the line of demarcation lies between one work and another may in fact be viewed differently from one culture to another. Consequently the bibliographic conventions established by various cultures or national groups may differ in terms of the criteria they use for determining the boundaries between one work and another. For the purposes of this model variant texts incorporating revisions or updates to an earlier text are viewed simply as expressions of the same work (i.e., the variant texts are not viewed as separate works). Similarly, abridgements or enlargements of an existing text, or the addition of parts or an accompaniment to a musical composition are considered to be different expressions of the same work. Translations from one language to another, musical transcriptions and arrangements, and dubbed or subtitled versions of a film are also considered simply as different expressions of the same original work. By contrast, when the modification of a work involves a significant degree of independent intellectual or artistic effort, the result is viewed, for the purpose of this model, as a new work. Thus paraphrases, rewritings, adaptations for children, parodies, musical variations on a theme and free transcriptions of a musical composition are considered to represent new works. Similarly, adaptations of a work from one literary or art form to another (e.g., dramatizations, adaptations from one medium of the graphic arts to another, etc.) are considered to represent new works. Abstracts, digests and summaries are also considered to represent new works. [Source: http://iflastandards.info/ns/fr/frbr/frbrer/C1001]</rdfs:comment>
        <rdfs:label xml:lang="en">Creative work</rdfs:label>
    </owl:Class>
    


    <!-- http://datos.bne.es/def/C1002 -->


    <owl:Class rdf:about="http://datos.bne.es/def/C1002">
        <rdfs:comment xml:lang="en">An expression is the specific intellectual or artistic form that a work takes each time it is &quot;realized&quot;. Expression encompasses, for example, the specific words, sentences, paragraphs, etc. that result from the realization of a work in the form of a text, or the particular sounds, phrasing, etc. resulting from the realization of a musical work. The boundaries of the entity expression are defined, however, so as to exclude aspects of physical form, such as typeface and page layout, that are not integral to the intellectual or artistic realization of the work as such. Inasmuch as the form of expression is an inherent characteristic of the expression, any change in form (e.g., from alpha-numeric notation to spoken word) results in a new expression. Similarly, changes in the intellectual conventions or instruments that are employed to express a work (e.g., translation from one language to another) result in the production of a new expression. If a text is revised or modified, the resulting expression is considered to be a new expression. The degree to which bibliographic distinctions are made between variant expressions of a work will depend to some extent on the nature of the work itself, on the anticipated needs of users and on what the cataloguer can reasonably be expected to recognize from the manifestation being described. Differences in form of expression (e.g., the differences between the expression of a work in the form of musical notation and the expression of the same work in the form of recorded sound) will normally be reflected in the bibliographic record, no matter what the nature of the work itself may be. Variant expressions in the same form (e.g., revised versions of a text) will often be indirectly identified as different expressions because the variation is apparent from the data associated with an attribute used to identify the manifestation in which the expression is embodied (e.g., an edition statement). Variations that would be evident only from a more detailed analysis and comparison of expressions (e.g., variations between several of the early texts of Shakespeare&apos;s Hamlet) would normally be reflected in the data only if the nature or stature of the work warranted such analysis, and only if it was anticipated that the distinction would be important to users. [Source: http://iflastandards.info/ns/fr/frbr/frbrer/C1002]</rdfs:comment>
        <rdfs:label xml:lang="en">Expression</rdfs:label>
    </owl:Class>
    


    <!-- http://datos.bne.es/def/C1003 -->


    <owl:Class rdf:about="http://datos.bne.es/def/C1003">
        <rdfs:comment xml:lang="en">An entity, tangible or intangible, that comprises intellectual and/or artistic content and is conceived, produced and/or issued as a unit, forming the basis of a single bibliographic description. Includes text, music, still and moving images, graphics, maps, sound recordings and video recordings, electronic data or programs, including those issued serially.[source: http://iflastandards.info/ns/isbd/elements/C2001]</rdfs:comment>
        <rdfs:comment xml:lang="es">Una entidad, tangible o intangible, que tiene contenido artístico y/o intelectual y que está concebida, producida y/o publicada como una unidad, formando la base de una descripción bibliográfica individual.  	Incluye texto, música, imágenes fijas y en movimiento, gráficos, mapas, grabaciones sonoras y videograbaciones, programas o datos electrónicos, incluyendo aquellos editados periódicamente. [fuente: ttp://iflastandards.info/ns/isbd/elements/C2001]</rdfs:comment>
        <rdfs:isDefinedBy>http://datos.bne.es/def/</rdfs:isDefinedBy>
        <rdfs:label xml:lang="es">Recurso</rdfs:label>
        <rdfs:label xml:lang="en">Resource</rdfs:label>
    </owl:Class>
    


    <!-- http://datos.bne.es/def/C1004 -->


    <owl:Class rdf:about="http://datos.bne.es/def/C1004">
        <rdfs:comment xml:lang="en">The entity defined as item is a concrete entity. It is in many instances a single physical object (e.g., a copy of a one-volume monograph, a single audio cassette, etc.). There are instances, however, where the entity defined as item comprises more than one physical object (e.g., a monograph issued as two separately bound volumes, a recording issued on three separate compact discs, etc.). In terms of intellectual content and physical form, an item exemplifying a manifestation is normally the same as the manifestation itself. However, variations may occur from one item to another, even when the items exemplify the same manifestation, where those variations are the result of actions external to the intent of the producer of the manifestation (e.g., damage occurring after the item was produced, binding performed by a library, etc.). [Source: http://iflastandards.info/ns/fr/frbr/frbrer/C1004]</rdfs:comment>
        <rdfs:label xml:lang="en">Item</rdfs:label>
    </owl:Class>
    


    <!-- http://datos.bne.es/def/C1005 -->


    <owl:Class rdf:about="http://datos.bne.es/def/C1005">
        <rdfs:comment xml:lang="en">The entity defined as person encompasses individuals that are deceased as well as those that are living. For the purposes of this model persons are treated as entities only to the extent that they are involved in the creation or realization of a work (e.g., as authors, composers, artists, editors, translators, directors, performers, etc.), or are the subject of a work (e.g., as the subject of a biographical or autobiographical work, of a history, etc.). [Source: http://iflastandards.info/ns/fr/frbr/frbrer/C1005]</rdfs:comment>
        <rdfs:label xml:lang="en">Person</rdfs:label>
    </owl:Class>
    


    <!-- http://datos.bne.es/def/C1006 -->


    <owl:Class rdf:about="http://datos.bne.es/def/C1006">
        <rdfs:comment xml:lang="en">The entity defined as corporate body encompasses organizations and groups of individuals and-or organizations that are identified by a particular name, including occasional groups and groups that are constituted as meetings, conferences, congresses, expeditions, exhibitions, festivals, fairs, etc. The entity also encompasses organizations that act as territorial authorities, exercising or claiming to exercise government functions over a certain territory, such as a federation, a state, a region, a local municipality, etc. The entity encompasses organizations and groups that are defunct as well as those that continue to operate.  For the purposes of this model corporate bodies are treated as entities only to the extent that they are involved in the creation or realization of a work (e.g., as the sponsors or endorsers of a work, etc.), or are the subject of a work (e.g., as the subject of a history, etc.). [Source: http://iflastandards.info/ns/fr/frbr/frbrer/C1006]</rdfs:comment>
        <rdfs:label xml:lang="en">Corporate Body</rdfs:label>
    </owl:Class>
    


    <!-- http://w3.id.org/def/BibliOWL#Cinema -->


    <owl:Class rdf:about="http://w3.id.org/def/BibliOWL#Cinema">
        <rdfs:subClassOf rdf:resource="http://datos.bne.es/def/C1001"/>
        <rdfs:label xml:lang="en">Cinematographic work</rdfs:label>
        <rdfs:label xml:lang="es">Obra cinematografica</rdfs:label>
    </owl:Class>
    


    <!-- http://w3.id.org/def/BibliOWL#Literature -->


    <owl:Class rdf:about="http://w3.id.org/def/BibliOWL#Literature">
        <rdfs:subClassOf rdf:resource="http://datos.bne.es/def/C1001"/>
        <rdfs:label xml:lang="en">Literacy work</rdfs:label>
        <rdfs:label xml:lang="es">Obra Literaria</rdfs:label>
    </owl:Class>
    


    <!-- http://w3.id.org/def/BibliOWL#Loan -->


    <owl:Class rdf:about="http://w3.id.org/def/BibliOWL#Loan">
        <rdfs:isDefinedBy>http://w3.id.org/def/BibliOWL#</rdfs:isDefinedBy>
        <rdfs:label xml:lang="en">Loan</rdfs:label>
    </owl:Class>
    


    <!-- http://w3.id.org/def/BibliOWL#Municipality -->


    <owl:Class rdf:about="http://w3.id.org/def/BibliOWL#Municipality">
        <rdfs:subClassOf rdf:resource="http://dati.beniculturali.it/cis/GovernamentalAdministrativeArea"/>
        <rdfs:isDefinedBy>http://w3.id.org/def/BibliOWL#</rdfs:isDefinedBy>
        <rdfs:label xml:lang="en">Municipality</rdfs:label>
    </owl:Class>
    


    <!-- http://w3.id.org/def/BibliOWL#Music -->


    <owl:Class rdf:about="http://w3.id.org/def/BibliOWL#Music">
        <rdfs:subClassOf rdf:resource="http://datos.bne.es/def/C1001"/>
        <rdfs:label xml:lang="en">Musical work</rdfs:label>
        <rdfs:label xml:lang="es">Obra musical</rdfs:label>
    </owl:Class>
    


    <!-- http://w3.id.org/def/BibliOWL#Province -->


    <owl:Class rdf:about="http://w3.id.org/def/BibliOWL#Province">
        <rdfs:subClassOf rdf:resource="http://dati.beniculturali.it/cis/GovernamentalAdministrativeArea"/>
        <rdfs:isDefinedBy>http://w3.id.org/def/BibliOWL#</rdfs:isDefinedBy>
        <rdfs:label xml:lang="en">Province</rdfs:label>
    </owl:Class>
    


    <!-- http://w3.id.org/def/BibliOWL#Region -->


    <owl:Class rdf:about="http://w3.id.org/def/BibliOWL#Region">
        <rdfs:subClassOf rdf:resource="http://dati.beniculturali.it/cis/GovernamentalAdministrativeArea"/>
        <rdfs:isDefinedBy>http://w3.id.org/def/BibliOWL#</rdfs:isDefinedBy>
        <rdfs:label xml:lang="en">Region</rdfs:label>
    </owl:Class>
    


    <!-- http://w3.id.org/def/BibliOWL#User -->


    <owl:Class rdf:about="http://w3.id.org/def/BibliOWL#User">
        <rdfs:subClassOf rdf:resource="http://datos.bne.es/def/C1005"/>
        <rdfs:label xml:lang="en">User</rdfs:label>
        <rdfs:label xml:lang="es">Usuario</rdfs:label>
    </owl:Class>
    


    <!-- http://w3.id.org/def/BibliOWL#UserOver18 -->


    <owl:Class rdf:about="http://w3.id.org/def/BibliOWL#UserOver18">
        <rdfs:subClassOf rdf:resource="http://w3.id.org/def/BibliOWL#UserType"/>
        <rdfs:isDefinedBy>http://w3.id.org/def/BibliOWL#</rdfs:isDefinedBy>
        <rdfs:label xml:lang="en">user over 18 years old</rdfs:label>
    </owl:Class>
    


    <!-- http://w3.id.org/def/BibliOWL#UserType -->


    <owl:Class rdf:about="http://w3.id.org/def/BibliOWL#UserType">
        <rdfs:isDefinedBy>http://w3.id.org/def/BibliOWL#</rdfs:isDefinedBy>
        <rdfs:label xml:lang="en">user type</rdfs:label>
    </owl:Class>
    


    <!-- http://w3.id.org/def/BibliOWL#UserUnder18 -->


    <owl:Class rdf:about="http://w3.id.org/def/BibliOWL#UserUnder18">
        <rdfs:subClassOf rdf:resource="http://w3.id.org/def/BibliOWL#UserType"/>
        <rdfs:isDefinedBy xml:lang="en">http://w3.id.org/def/BibliOWL#</rdfs:isDefinedBy>
        <rdfs:label xml:lang="en">user under 18 years old</rdfs:label>
    </owl:Class>
    


    <!-- http://www.rdaregistry.info/termList/RDAContentType/#1003 -->


    <owl:Class rdf:about="http://www.rdaregistry.info/termList/RDAContentType/#1003">
        <rdfs:subClassOf rdf:resource="http://datos.bne.es/def/C1002"/>
        <rdfs:comment xml:lang="en">A content type that consists of cartographic content expressed through images intended to be perceived as moving, in two dimensions.</rdfs:comment>
        <rdfs:label xml:lang="en">cartographic moving image</rdfs:label>
    </owl:Class>
    


    <!-- http://www.rdaregistry.info/termList/RDAContentType/#1010 -->


    <owl:Class rdf:about="http://www.rdaregistry.info/termList/RDAContentType/#1010">
        <rdfs:subClassOf rdf:resource="http://datos.bne.es/def/C1002"/>
        <rdfs:comment xml:lang="en">A content type that consists of content expressed through a form of musical notation intended to be perceived visually</rdfs:comment>
        <rdfs:label xml:lang="en">Notated music</rdfs:label>
    </owl:Class>
    


    <!-- http://www.rdaregistry.info/termList/RDAContentType/#1011 -->


    <owl:Class rdf:about="http://www.rdaregistry.info/termList/RDAContentType/#1011">
        <rdfs:subClassOf rdf:resource="http://datos.bne.es/def/C1002"/>
        <rdfs:comment xml:lang="en">A content type that consists of content expressed through music in an audible form.</rdfs:comment>
        <rdfs:label xml:lang="en">Performed music</rdfs:label>
    </owl:Class>
    


    <!-- http://www.rdaregistry.info/termList/RDAContentType/#1012 -->


    <owl:Class rdf:about="http://www.rdaregistry.info/termList/RDAContentType/#1012">
        <rdfs:subClassOf rdf:resource="http://datos.bne.es/def/C1002"/>
        <rdfs:comment xml:lang="en">A content type that consists of content other than language or music, expressed in an audible form.</rdfs:comment>
        <rdfs:label xml:lang="en">sounds</rdfs:label>
    </owl:Class>
    


    <!-- http://www.rdaregistry.info/termList/RDAContentType/#1013 -->


    <owl:Class rdf:about="http://www.rdaregistry.info/termList/RDAContentType/#1013">
        <rdfs:subClassOf rdf:resource="http://datos.bne.es/def/C1002"/>
        <rdfs:comment xml:lang="en">A content type that consists of content expressed through language in an audible form.</rdfs:comment>
        <rdfs:label xml:lang="en">Spoken word</rdfs:label>
    </owl:Class>
    


    <!-- http://www.rdaregistry.info/termList/RDAContentType/#1020 -->


    <owl:Class rdf:about="http://www.rdaregistry.info/termList/RDAContentType/#1020">
        <rdfs:subClassOf rdf:resource="http://datos.bne.es/def/C1002"/>
        <rdfs:comment xml:lang="en">A content type that consists of content expressed through a form of notation for language intended to be perceived visually</rdfs:comment>
        <rdfs:label xml:lang="en">Text</rdfs:label>
    </owl:Class>
    


    <!-- http://www.rdaregistry.info/termList/RDAContentType/#1023 -->


    <owl:Class rdf:about="http://www.rdaregistry.info/termList/RDAContentType/#1023">
        <rdfs:subClassOf rdf:resource="http://datos.bne.es/def/C1002"/>
        <rdfs:comment xml:lang="en">A content type that consists of content expressed through images intended to be perceived to be moving, and in two dimensions</rdfs:comment>
        <rdfs:label xml:lang="en">two-dimensional moving image</rdfs:label>
    </owl:Class>
    


    <!-- http://www.w3.org/2002/07/owl#Thing -->


    <owl:Class rdf:about="http://www.w3.org/2002/07/owl#Thing"/>
    


    <!-- 
    ///////////////////////////////////////////////////////////////////////////////////////
    //
    // Individuals
    //
    ///////////////////////////////////////////////////////////////////////////////////////
     -->


    


    <!-- http://dati.beniculturali.it/cis/ -->


    <owl:NamedIndividual rdf:about="http://dati.beniculturali.it/cis/"/>
    


    <!-- http://dati.beniculturali.it/cis/Friday -->


    <owl:NamedIndividual rdf:about="http://dati.beniculturali.it/cis/Friday">
        <rdf:type rdf:resource="http://dati.beniculturali.it/cis/DayOfWeek"/>
        <rdfs:label xml:lang="en">Friday</rdfs:label>
        <rdfs:label xml:lang="it">Venerdì</rdfs:label>
    </owl:NamedIndividual>
    


    <!-- http://dati.beniculturali.it/cis/Monday -->


    <owl:NamedIndividual rdf:about="http://dati.beniculturali.it/cis/Monday">
        <rdf:type rdf:resource="http://dati.beniculturali.it/cis/DayOfWeek"/>
        <rdfs:label xml:lang="it">Lunedì </rdfs:label>
        <rdfs:label xml:lang="en">Monday </rdfs:label>
    </owl:NamedIndividual>
    


    <!-- http://dati.beniculturali.it/cis/Saturday -->


    <owl:NamedIndividual rdf:about="http://dati.beniculturali.it/cis/Saturday">
        <rdf:type rdf:resource="http://dati.beniculturali.it/cis/DayOfWeek"/>
        <rdfs:label xml:lang="it">Sabato</rdfs:label>
        <rdfs:label xml:lang="en">Saturday</rdfs:label>
    </owl:NamedIndividual>
    


    <!-- http://dati.beniculturali.it/cis/Sunday -->


    <owl:NamedIndividual rdf:about="http://dati.beniculturali.it/cis/Sunday">
        <rdf:type rdf:resource="http://dati.beniculturali.it/cis/DayOfWeek"/>
        <rdfs:label xml:lang="it">Domenica</rdfs:label>
        <rdfs:label xml:lang="en">Sunday</rdfs:label>
    </owl:NamedIndividual>
    


    <!-- http://dati.beniculturali.it/cis/Thursday -->


    <owl:NamedIndividual rdf:about="http://dati.beniculturali.it/cis/Thursday">
        <rdf:type rdf:resource="http://dati.beniculturali.it/cis/DayOfWeek"/>
        <rdfs:label xml:lang="it">Giovedì </rdfs:label>
        <rdfs:label xml:lang="en">Thursday </rdfs:label>
    </owl:NamedIndividual>
    


    <!-- http://dati.beniculturali.it/cis/Tuesday -->


    <owl:NamedIndividual rdf:about="http://dati.beniculturali.it/cis/Tuesday">
        <rdf:type rdf:resource="http://dati.beniculturali.it/cis/DayOfWeek"/>
        <rdfs:label xml:lang="it">Martedì</rdfs:label>
        <rdfs:label xml:lang="en">Tuesday</rdfs:label>
    </owl:NamedIndividual>
    


    <!-- http://dati.beniculturali.it/cis/Wednesday -->


    <owl:NamedIndividual rdf:about="http://dati.beniculturali.it/cis/Wednesday">
        <rdf:type rdf:resource="http://dati.beniculturali.it/cis/DayOfWeek"/>
        <rdfs:label xml:lang="it">Mercoledì</rdfs:label>
        <rdfs:label xml:lang="en">Wednesday</rdfs:label>
    </owl:NamedIndividual>
    


    <!-- http://w3.id.org/def/BibliOWL#AlvaroGonzalezBerdasco -->


    <owl:NamedIndividual rdf:about="http://w3.id.org/def/BibliOWL#AlvaroGonzalezBerdasco">
        <rdf:type rdf:resource="http://w3.id.org/def/BibliOWL#User"/>
        <hasUserType rdf:resource="http://w3.id.org/def/BibliOWL#User18-25"/>
        <isUserOf rdf:resource="http://w3.id.org/def/BibliOWL#BPMBenicarlo"/>
        <participatesAtLoan rdf:resource="http://w3.id.org/def/BibliOWL#Loan0001AAA"/>
        <def:P5001 rdf:datatype="http://www.w3.org/2000/01/rdf-schema#Literal">Álvaro González Berdasco</def:P5001>
        <def:P5010 rdf:datatype="http://www.w3.org/2001/XMLSchema#date">1999-11-08</def:P5010>
        <userID rdf:datatype="http://www.w3.org/2000/01/rdf-schema#Literal">AGB000001</userID>
    </owl:NamedIndividual>
    


    <!-- http://w3.id.org/def/BibliOWL#BPMBenicarlo -->


    <owl:NamedIndividual rdf:about="http://w3.id.org/def/BibliOWL#BPMBenicarlo">
        <rdf:type rdf:resource="http://dati.beniculturali.it/cis/Library"/>
        <cis:catalogue rdf:resource="http://w3.id.org/def/BibliOWL#BPMBenicarloCatalogue"/>
        <cis:hasAccessCondition rdf:resource="http://w3.id.org/def/BibliOWL#BPMBenicarloOHSSaturday"/>
        <cis:hasAccessCondition rdf:resource="http://w3.id.org/def/BibliOWL#BPMBenicarloOHSWeek"/>
        <cis:hasAccessCondition rdf:resource="http://w3.id.org/def/BibliOWL#FloorRenovation"/>
        <cis:hasContactPoint rdf:resource="http://w3.id.org/def/BibliOWL#BPMBenicarloContact"/>
        <cis:hasSite rdf:resource="http://w3.id.org/def/BibliOWL#BPMBenicarloSite"/>
        <cis:providesService rdf:resource="http://w3.id.org/def/BibliOWL#InternetAccess"/>
        <cis:ISILIdentifier rdf:datatype="http://www.w3.org/2000/01/rdf-schema#Literal">13ln84fcs96ljr</cis:ISILIdentifier>
        <cis:hasWebSite rdf:datatype="http://www.w3.org/2001/XMLSchema#anyURI">http://www.ajuntamentdebenicarlo.org/bib/pbib-biblioteca.php3?g_idioma=v</cis:hasWebSite>
        <cis:institutionalName rdf:datatype="http://www.w3.org/2000/01/rdf-schema#Literal">Biblioteca Pública Municipal Manuel García I Benicarló</cis:institutionalName>
    </owl:NamedIndividual>
    


    <!-- http://w3.id.org/def/BibliOWL#BPMBenicarloAddress -->


    <owl:NamedIndividual rdf:about="http://w3.id.org/def/BibliOWL#BPMBenicarloAddress">
        <rdf:type rdf:resource="http://dati.beniculturali.it/cis/Address"/>
        <cis:addressID rdf:datatype="http://www.w3.org/2000/01/rdf-schema#Literal">5840jdel9uf</cis:addressID>
        <cis:fullAddress rdf:datatype="http://www.w3.org/2000/01/rdf-schema#Literal">Carrer de Peníscola, 21, 12580 Benicarló, Castelló</cis:fullAddress>
        <cis:postCode rdf:datatype="http://www.w3.org/2000/01/rdf-schema#Literal">12580</cis:postCode>
    </owl:NamedIndividual>
    


    <!-- http://w3.id.org/def/BibliOWL#BPMBenicarloCatalogue -->


    <owl:NamedIndividual rdf:about="http://w3.id.org/def/BibliOWL#BPMBenicarloCatalogue">
        <rdf:type rdf:resource="http://dati.beniculturali.it/cis/Catalogue"/>
        <contains rdf:resource="http://w3.id.org/def/BibliOWL#SMBM34A01"/>
    </owl:NamedIndividual>
    


    <!-- http://w3.id.org/def/BibliOWL#BPMBenicarloContact -->


    <owl:NamedIndividual rdf:about="http://w3.id.org/def/BibliOWL#BPMBenicarloContact">
        <rdf:type rdf:resource="http://dati.beniculturali.it/cis/ContactPoint"/>
        <cis:available rdf:resource="http://w3.id.org/def/BibliOWL#BPMBenicarloOHSSaturday"/>
        <cis:available rdf:resource="http://w3.id.org/def/BibliOWL#BPMBenicarloOHSWeek"/>
        <cis:hasEmail rdf:datatype="http://www.w3.org/2001/XMLSchema#anyURI">correu.biblioteca@ajuntamentdebenicarlo.org</cis:hasEmail>
        <cis:hasTelephone rdf:datatype="http://www.w3.org/2000/01/rdf-schema#Literal">964475660</cis:hasTelephone>
    </owl:NamedIndividual>
    


    <!-- http://w3.id.org/def/BibliOWL#BPMBenicarloGeometry -->


    <owl:NamedIndividual rdf:about="http://w3.id.org/def/BibliOWL#BPMBenicarloGeometry">
        <rdf:type rdf:resource="http://dati.beniculturali.it/cis/Geometry"/>
        <cis:hasLat rdf:datatype="http://www.w3.org/2000/01/rdf-schema#Literal">40.414282</cis:hasLat>
        <cis:hasLong rdf:datatype="http://www.w3.org/2000/01/rdf-schema#Literal">0.423415</cis:hasLong>
    </owl:NamedIndividual>
    


    <!-- http://w3.id.org/def/BibliOWL#BPMBenicarloOHSSaturday -->


    <owl:NamedIndividual rdf:about="http://w3.id.org/def/BibliOWL#BPMBenicarloOHSSaturday">
        <rdf:type rdf:resource="http://dati.beniculturali.it/cis/OpeningHoursSpecification"/>
        <cis:hasDayOfWeek rdf:resource="http://dati.beniculturali.it/cis/Saturday"/>
        <cis:closes rdf:datatype="http://www.w3.org/2001/XMLSchema#time">13:30</cis:closes>
        <cis:opens rdf:datatype="http://www.w3.org/2001/XMLSchema#time">09:30</cis:opens>
    </owl:NamedIndividual>
    


    <!-- http://w3.id.org/def/BibliOWL#BPMBenicarloOHSWeek -->


    <owl:NamedIndividual rdf:about="http://w3.id.org/def/BibliOWL#BPMBenicarloOHSWeek">
        <rdf:type rdf:resource="http://dati.beniculturali.it/cis/OpeningHoursSpecification"/>
        <cis:hasDayOfWeek rdf:resource="http://w3.id.org/def/BibliOWL#WeekDays"/>
        <cis:closes rdf:datatype="http://www.w3.org/2001/XMLSchema#time">20:00</cis:closes>
        <cis:opens rdf:datatype="http://www.w3.org/2001/XMLSchema#time">09:00</cis:opens>
    </owl:NamedIndividual>
    


    <!-- http://w3.id.org/def/BibliOWL#BPMBenicarloSite -->


    <owl:NamedIndividual rdf:about="http://w3.id.org/def/BibliOWL#BPMBenicarloSite">
        <rdf:type rdf:resource="http://dati.beniculturali.it/cis/Site"/>
        <cis:hasAddress rdf:resource="http://w3.id.org/def/BibliOWL#BPMBenicarloAddress"/>
        <cis:hasGeographicalLocation rdf:resource="http://w3.id.org/def/BibliOWL#Benicarlo"/>
        <cis:hasGeometry rdf:resource="http://w3.id.org/def/BibliOWL#BPMBenicarloGeometry"/>
    </owl:NamedIndividual>
    


    <!-- http://w3.id.org/def/BibliOWL#Benicarlo -->


    <owl:NamedIndividual rdf:about="http://w3.id.org/def/BibliOWL#Benicarlo">
        <rdf:type rdf:resource="http://w3.id.org/def/BibliOWL#Municipality"/>
        <obo:BFO_0000050 rdf:resource="http://w3.id.org/def/BibliOWL#Castellon"/>
        <cis:toponym rdf:datatype="http://www.w3.org/2000/01/rdf-schema#Literal">Benicarló</cis:toponym>
    </owl:NamedIndividual>
    


    <!-- http://w3.id.org/def/BibliOWL#Castellon -->


    <owl:NamedIndividual rdf:about="http://w3.id.org/def/BibliOWL#Castellon">
        <rdf:type rdf:resource="http://w3.id.org/def/BibliOWL#Province"/>
        <obo:BFO_0000050 rdf:resource="http://w3.id.org/def/BibliOWL#ComunidadValenciana"/>
        <cis:toponym rdf:datatype="http://www.w3.org/2000/01/rdf-schema#Literal">Castellón</cis:toponym>
    </owl:NamedIndividual>
    


    <!-- http://w3.id.org/def/BibliOWL#ComunidadValenciana -->


    <owl:NamedIndividual rdf:about="http://w3.id.org/def/BibliOWL#ComunidadValenciana">
        <rdf:type rdf:resource="http://w3.id.org/def/BibliOWL#Region"/>
        <cis:toponym rdf:datatype="http://www.w3.org/2000/01/rdf-schema#Literal">Comunidad Valenciana</cis:toponym>
    </owl:NamedIndividual>
    


    <!-- http://w3.id.org/def/BibliOWL#FloorRenovation -->


    <owl:NamedIndividual rdf:about="http://w3.id.org/def/BibliOWL#FloorRenovation">
        <rdf:type rdf:resource="http://dati.beniculturali.it/cis/TemporaryClosure"/>
        <hasTimeInterval rdf:resource="http://w3.id.org/def/BibliOWL#RenovationPeriod"/>
        <cis:hasReason rdf:datatype="http://www.w3.org/2000/01/rdf-schema#Literal">Period of time for fixing the bulding&apos;s floor.</cis:hasReason>
    </owl:NamedIndividual>
    


    <!-- http://w3.id.org/def/BibliOWL#GrupoAnaya -->


    <owl:NamedIndividual rdf:about="http://w3.id.org/def/BibliOWL#GrupoAnaya">
        <rdf:type rdf:resource="http://datos.bne.es/def/C1006"/>
        <def:OP6004 rdf:resource="http://w3.id.org/def/BibliOWL#SMBM34A"/>
        <corporateBodyName rdf:datatype="http://www.w3.org/2000/01/rdf-schema#Literal">Grupo Anaya, S.A.</corporateBodyName>
    </owl:NamedIndividual>
    


    <!-- http://w3.id.org/def/BibliOWL#InternetAccess -->


    <owl:NamedIndividual rdf:about="http://w3.id.org/def/BibliOWL#InternetAccess">
        <rdf:type rdf:resource="http://dati.beniculturali.it/cis/Service"/>
    </owl:NamedIndividual>
    


    <!-- http://w3.id.org/def/BibliOWL#Loan0001AAA -->


    <owl:NamedIndividual rdf:about="http://w3.id.org/def/BibliOWL#Loan0001AAA">
        <rdf:type rdf:resource="http://w3.id.org/def/BibliOWL#Loan"/>
        <validDuring rdf:resource="http://w3.id.org/def/BibliOWL#LoanAAA0001"/>
        <loanID rdf:datatype="http://www.w3.org/2000/01/rdf-schema#Literal">0001AAA</loanID>
    </owl:NamedIndividual>
    


    <!-- http://w3.id.org/def/BibliOWL#LoanAAA0001 -->


    <owl:NamedIndividual rdf:about="http://w3.id.org/def/BibliOWL#LoanAAA0001">
        <rdf:type rdf:resource="http://dati.beniculturali.it/cis/TimeInterval"/>
        <cis:endDate rdf:datatype="http://www.w3.org/2001/XMLSchema#date">2023-01-25</cis:endDate>
        <cis:startDate rdf:datatype="http://www.w3.org/2001/XMLSchema#date">2023-01-20</cis:startDate>
    </owl:NamedIndividual>
    


    <!-- http://w3.id.org/def/BibliOWL#MarioValdes -->


    <owl:NamedIndividual rdf:about="http://w3.id.org/def/BibliOWL#MarioValdes">
        <rdf:type rdf:resource="http://datos.bne.es/def/C1005"/>
        <def:OP3005 rdf:resource="http://w3.id.org/def/BibliOWL#SMBM34A"/>
        <def:P5001 rdf:datatype="http://www.w3.org/2000/01/rdf-schema#Literal">Mario J. Valdés</def:P5001>
        <def:P5010 rdf:datatype="http://www.w3.org/2001/XMLSchema#date">1934-01-28</def:P5010>
        <def:P5011 rdf:datatype="http://www.w3.org/2001/XMLSchema#date">2020-04-26</def:P5011>
    </owl:NamedIndividual>
    


    <!-- http://w3.id.org/def/BibliOWL#MiguelDeUnamuno -->


    <owl:NamedIndividual rdf:about="http://w3.id.org/def/BibliOWL#MiguelDeUnamuno">
        <rdf:type rdf:resource="http://datos.bne.es/def/C1005"/>
        <def:P5001 rdf:datatype="http://www.w3.org/2000/01/rdf-schema#Literal">Miguel de Unamuno y Jugo</def:P5001>
        <def:P5005 rdf:datatype="http://www.w3.org/2001/XMLSchema#anyURI">https://www.biografiasyvidas.com/biografia/u/unamuno.htm</def:P5005>
        <def:P5008 rdf:datatype="http://www.w3.org/2000/01/rdf-schema#Literal">Miguel de Unamuno</def:P5008>
        <def:P5010 rdf:datatype="http://www.w3.org/2001/XMLSchema#date">1864-09-29</def:P5010>
        <def:P5011 rdf:datatype="http://www.w3.org/2001/XMLSchema#date">1936-12-31</def:P5011>
    </owl:NamedIndividual>
    


    <!-- http://w3.id.org/def/BibliOWL#RenovationPeriod -->


    <owl:NamedIndividual rdf:about="http://w3.id.org/def/BibliOWL#RenovationPeriod">
        <rdf:type rdf:resource="http://dati.beniculturali.it/cis/TimeInterval"/>
        <cis:endDate rdf:datatype="http://www.w3.org/2001/XMLSchema#dateTime">2023-05-30T23:59:00</cis:endDate>
        <cis:startDate rdf:datatype="http://www.w3.org/2001/XMLSchema#dateTime">2023-05-10T00:00:00</cis:startDate>
    </owl:NamedIndividual>
    


    <!-- http://w3.id.org/def/BibliOWL#SMBM -->


    <owl:NamedIndividual rdf:about="http://w3.id.org/def/BibliOWL#SMBM">
        <rdf:type rdf:resource="http://w3.id.org/def/BibliOWL#Literature"/>
        <def:OP1001 rdf:resource="http://w3.id.org/def/BibliOWL#MiguelDeUnamuno"/>
        <def:P1001 rdf:datatype="http://www.w3.org/2000/01/rdf-schema#Literal">San Manuel Bueno, mártir</def:P1001>
        <def:P1004 rdf:datatype="http://www.w3.org/2001/XMLSchema#date">1931</def:P1004>
        <hasGenre rdf:datatype="http://www.w3.org/2000/01/rdf-schema#Literal">Novela</hasGenre>
    </owl:NamedIndividual>
    


    <!-- http://w3.id.org/def/BibliOWL#SMBM34A -->


    <owl:NamedIndividual rdf:about="http://w3.id.org/def/BibliOWL#SMBM34A">
        <rdf:type rdf:resource="http://datos.bne.es/def/C1003"/>
        <def:OP3001 rdf:resource="http://w3.id.org/def/BibliOWL#SMBM34A01"/>
        <def:P3004 rdf:datatype="http://www.w3.org/2000/01/rdf-schema#Literal">Book</def:P3004>
        <def:P3013 rdf:datatype="http://www.w3.org/2000/01/rdf-schema#Literal">978-84-376-0185-4</def:P3013>
        <def:P3015 rdf:datatype="http://www.w3.org/2000/01/rdf-schema#Literal">The book comes with an audiobook in CD format.</def:P3015>
        <def:P3048 rdf:datatype="http://www.w3.org/2001/XMLSchema#date">2014</def:P3048>
        <hasAppropiateAge rdf:datatype="http://www.w3.org/2001/XMLSchema#int">14</hasAppropiateAge>
        <rdfs:comment rdf:datatype="http://www.w3.org/2000/01/rdf-schema#Literal">San Manuel Bueno, Mártir 34th edition. Miguel de Unamuno. Edited by Mario Valdés. Ediciones Cátedra (Grupo Anaya)</rdfs:comment>
    </owl:NamedIndividual>
    


    <!-- http://w3.id.org/def/BibliOWL#SMBM34A01 -->


    <owl:NamedIndividual rdf:about="http://w3.id.org/def/BibliOWL#SMBM34A01">
        <rdf:type rdf:resource="http://datos.bne.es/def/C1004"/>
        <isBorrowedAtLoan rdf:resource="http://w3.id.org/def/BibliOWL#Loan0001AAA"/>
        <itemID rdf:datatype="http://www.w3.org/2000/01/rdf-schema#Literal">SMBM34A01</itemID>
    </owl:NamedIndividual>
    


    <!-- http://w3.id.org/def/BibliOWL#SMBMBookSp -->


    <owl:NamedIndividual rdf:about="http://w3.id.org/def/BibliOWL#SMBMBookSp">
        <rdf:type rdf:resource="http://www.rdaregistry.info/termList/RDAContentType/#1020"/>
        <def:OP2001 rdf:resource="http://w3.id.org/def/BibliOWL#SMBM34A"/>
        <def:OP2002 rdf:resource="http://w3.id.org/def/BibliOWL#SMBM"/>
        <def:P2001 rdf:datatype="http://www.w3.org/2000/01/rdf-schema#Literal">Spanish</def:P2001>
    </owl:NamedIndividual>
    


    <!-- http://w3.id.org/def/BibliOWL#User15-18 -->


    <owl:NamedIndividual rdf:about="http://w3.id.org/def/BibliOWL#User15-18">
        <rdf:type rdf:resource="http://w3.id.org/def/BibliOWL#UserUnder18"/>
    </owl:NamedIndividual>
    


    <!-- http://w3.id.org/def/BibliOWL#User18-25 -->


    <owl:NamedIndividual rdf:about="http://w3.id.org/def/BibliOWL#User18-25">
        <rdf:type rdf:resource="http://w3.id.org/def/BibliOWL#UserOver18"/>
    </owl:NamedIndividual>
    


    <!-- http://w3.id.org/def/BibliOWL#User26-40 -->


    <owl:NamedIndividual rdf:about="http://w3.id.org/def/BibliOWL#User26-40">
        <rdf:type rdf:resource="http://w3.id.org/def/BibliOWL#UserOver18"/>
    </owl:NamedIndividual>
    


    <!-- http://w3.id.org/def/BibliOWL#User41-65 -->


    <owl:NamedIndividual rdf:about="http://w3.id.org/def/BibliOWL#User41-65">
        <rdf:type rdf:resource="http://w3.id.org/def/BibliOWL#UserOver18"/>
    </owl:NamedIndividual>
    


    <!-- http://w3.id.org/def/BibliOWL#User66- -->


    <owl:NamedIndividual rdf:about="http://w3.id.org/def/BibliOWL#User66-">
        <rdf:type rdf:resource="http://w3.id.org/def/BibliOWL#UserOver18"/>
    </owl:NamedIndividual>
    


    <!-- http://w3.id.org/def/BibliOWL#WeekDays -->


    <owl:NamedIndividual rdf:about="http://w3.id.org/def/BibliOWL#WeekDays">
        <rdf:type rdf:resource="http://dati.beniculturali.it/cis/DayOfWeek"/>
        <rdfs:comment rdf:datatype="http://www.w3.org/2000/01/rdf-schema#Literal">Includes days of the week from Monday to Friday</rdfs:comment>
    </owl:NamedIndividual>
    


    <!-- http://w3.id.org/def/BibliOWL#Weekend -->


    <owl:NamedIndividual rdf:about="http://w3.id.org/def/BibliOWL#Weekend">
        <rdf:type rdf:resource="http://dati.beniculturali.it/cis/DayOfWeek"/>
    </owl:NamedIndividual>
    


    <!-- 
    ///////////////////////////////////////////////////////////////////////////////////////
    //
    // General axioms
    //
    ///////////////////////////////////////////////////////////////////////////////////////
     -->


    <rdf:Description>
        <rdf:type rdf:resource="http://www.w3.org/2002/07/owl#AllDisjointClasses"/>
        <owl:members rdf:parseType="Collection">
            <rdf:Description rdf:about="http://w3.id.org/def/BibliOWL#Cinema"/>
            <rdf:Description rdf:about="http://w3.id.org/def/BibliOWL#Literature"/>
            <rdf:Description rdf:about="http://w3.id.org/def/BibliOWL#Music"/>
        </owl:members>
    </rdf:Description>
    <rdf:Description>
        <rdf:type rdf:resource="http://www.w3.org/2002/07/owl#AllDisjointClasses"/>
        <owl:members rdf:parseType="Collection">
            <rdf:Description rdf:about="http://w3.id.org/def/BibliOWL#Municipality"/>
            <rdf:Description rdf:about="http://w3.id.org/def/BibliOWL#Province"/>
            <rdf:Description rdf:about="http://w3.id.org/def/BibliOWL#Region"/>
        </owl:members>
    </rdf:Description>
</rdf:RDF>



<!-- Generated by the OWL API (version 5.1.18) https://github.com/owlcs/owlapi/ -->


